x86/proofs/mlkem_basemul_k2.ml
@@ -1,0 +1,1456 @@
+(*
+ * Copyright Amazon.com, Inc. or its affiliates. All Rights Reserved.
+ * SPDX-License-Identifier: Apache-2.0 OR ISC OR MIT-0
+ *)
+
+(* ========================================================================= *)
+(* Scalar multiplication of 2-element polynomial vectors in NTT domain.      *)
+(* ========================================================================= *)
+
+needs "x86/proofs/base.ml";;
+needs "common/mlkem_mldsa.ml";;
+
+print_literal_from_elf "x86/mlkem/mlkem_basemul_k2.o";;
+
+let mlkem_basemul_k2_mc =
+  define_assert_from_elf "mlkem_basemul_k2_mc" "x86/mlkem/mlkem_basemul_k2.o"
+[
+  0xf3; 0x0f; 0x1e; 0xfa;  (* ENDBR64 *)
+  0xb8; 0x01; 0x0d; 0x01; 0x0d;
+                           (* MOV (% eax) (Imm32 (word 218172673)) *)
+  0xc5; 0xf9; 0x6e; 0xc0;  (* VMOVD (%_% xmm0) (% eax) *)
+  0xc4; 0xe2; 0x7d; 0x58; 0xc0;
+                           (* VPBROADCASTD (%_% ymm0) (%_% xmm0) *)
+  0xb8; 0x01; 0xf3; 0x01; 0xf3;
+                           (* MOV (% eax) (Imm32 (word 4076991233)) *)
+  0xc5; 0xf9; 0x6e; 0xc8;  (* VMOVD (%_% xmm1) (% eax) *)
+  0xc4; 0xe2; 0x7d; 0x58; 0xc9;
+                           (* VPBROADCASTD (%_% ymm1) (%_% xmm1) *)
+  0xc5; 0xfd; 0x6f; 0x16;  (* VMOVDQA (%_% ymm2) (Memop Word256 (%% (rsi,0))) *)
+  0xc5; 0xfd; 0x6f; 0x5e; 0x20;
+                           (* VMOVDQA (%_% ymm3) (Memop Word256 (%% (rsi,32))) *)
+  0xc5; 0xfd; 0x6f; 0x22;  (* VMOVDQA (%_% ymm4) (Memop Word256 (%% (rdx,0))) *)
+  0xc5; 0xfd; 0x6f; 0x6a; 0x20;
+                           (* VMOVDQA (%_% ymm5) (Memop Word256 (%% (rdx,32))) *)
+  0xc5; 0xfd; 0x6f; 0x31;  (* VMOVDQA (%_% ymm6) (Memop Word256 (%% (rcx,0))) *)
+  0xc5; 0x75; 0xd5; 0xea;  (* VPMULLW (%_% ymm13) (%_% ymm1) (%_% ymm2) *)
+  0xc5; 0x75; 0xd5; 0xf3;  (* VPMULLW (%_% ymm14) (%_% ymm1) (%_% ymm3) *)
+  0xc4; 0xc1; 0x5d; 0xd5; 0xfd;
+                           (* VPMULLW (%_% ymm7) (%_% ymm4) (%_% ymm13) *)
+  0xc4; 0x41; 0x55; 0xd5; 0xcd;
+                           (* VPMULLW (%_% ymm9) (%_% ymm5) (%_% ymm13) *)
+  0xc4; 0x41; 0x4d; 0xd5; 0xc6;
+                           (* VPMULLW (%_% ymm8) (%_% ymm6) (%_% ymm14) *)
+  0xc4; 0x41; 0x5d; 0xd5; 0xd6;
+                           (* VPMULLW (%_% ymm10) (%_% ymm4) (%_% ymm14) *)
+  0xc5; 0xfd; 0xe5; 0xff;  (* VPMULHW (%_% ymm7) (%_% ymm0) (%_% ymm7) *)
+  0xc4; 0x41; 0x7d; 0xe5; 0xc9;
+                           (* VPMULHW (%_% ymm9) (%_% ymm0) (%_% ymm9) *)
+  0xc4; 0x41; 0x7d; 0xe5; 0xc0;
+                           (* VPMULHW (%_% ymm8) (%_% ymm0) (%_% ymm8) *)
+  0xc4; 0x41; 0x7d; 0xe5; 0xd2;
+                           (* VPMULHW (%_% ymm10) (%_% ymm0) (%_% ymm10) *)
+  0xc5; 0x5d; 0xe5; 0xda;  (* VPMULHW (%_% ymm11) (%_% ymm4) (%_% ymm2) *)
+  0xc5; 0x55; 0xe5; 0xe2;  (* VPMULHW (%_% ymm12) (%_% ymm5) (%_% ymm2) *)
+  0xc5; 0x4d; 0xe5; 0xeb;  (* VPMULHW (%_% ymm13) (%_% ymm6) (%_% ymm3) *)
+  0xc5; 0x5d; 0xe5; 0xf3;  (* VPMULHW (%_% ymm14) (%_% ymm4) (%_% ymm3) *)
+  0xc5; 0xa5; 0xf9; 0xff;  (* VPSUBW (%_% ymm7) (%_% ymm11) (%_% ymm7) *)
+  0xc4; 0x41; 0x1d; 0xf9; 0xc9;
+                           (* VPSUBW (%_% ymm9) (%_% ymm12) (%_% ymm9) *)
+  0xc4; 0x41; 0x15; 0xf9; 0xc0;
+                           (* VPSUBW (%_% ymm8) (%_% ymm13) (%_% ymm8) *)
+  0xc4; 0x41; 0x0d; 0xf9; 0xd2;
+                           (* VPSUBW (%_% ymm10) (%_% ymm14) (%_% ymm10) *)
+  0xc5; 0xbd; 0xfd; 0xff;  (* VPADDW (%_% ymm7) (%_% ymm8) (%_% ymm7) *)
+  0xc4; 0x41; 0x2d; 0xfd; 0xc9;
+                           (* VPADDW (%_% ymm9) (%_% ymm10) (%_% ymm9) *)
+  0xc5; 0xfd; 0x7f; 0x3f;  (* VMOVDQA (Memop Word256 (%% (rdi,0))) (%_% ymm7) *)
+  0xc5; 0x7d; 0x7f; 0x4f; 0x20;
+                           (* VMOVDQA (Memop Word256 (%% (rdi,32))) (%_% ymm9) *)
+  0xc5; 0xfd; 0x6f; 0x56; 0x40;
+                           (* VMOVDQA (%_% ymm2) (Memop Word256 (%% (rsi,64))) *)
+  0xc5; 0xfd; 0x6f; 0x5e; 0x60;
+                           (* VMOVDQA (%_% ymm3) (Memop Word256 (%% (rsi,96))) *)
+  0xc5; 0xfd; 0x6f; 0x62; 0x40;
+                           (* VMOVDQA (%_% ymm4) (Memop Word256 (%% (rdx,64))) *)
+  0xc5; 0xfd; 0x6f; 0x6a; 0x60;
+                           (* VMOVDQA (%_% ymm5) (Memop Word256 (%% (rdx,96))) *)
+  0xc5; 0xfd; 0x6f; 0x71; 0x20;
+                           (* VMOVDQA (%_% ymm6) (Memop Word256 (%% (rcx,32))) *)
+  0xc5; 0x75; 0xd5; 0xea;  (* VPMULLW (%_% ymm13) (%_% ymm1) (%_% ymm2) *)
+  0xc5; 0x75; 0xd5; 0xf3;  (* VPMULLW (%_% ymm14) (%_% ymm1) (%_% ymm3) *)
+  0xc4; 0xc1; 0x5d; 0xd5; 0xfd;
+                           (* VPMULLW (%_% ymm7) (%_% ymm4) (%_% ymm13) *)
+  0xc4; 0x41; 0x55; 0xd5; 0xcd;
+                           (* VPMULLW (%_% ymm9) (%_% ymm5) (%_% ymm13) *)
+  0xc4; 0x41; 0x4d; 0xd5; 0xc6;
+                           (* VPMULLW (%_% ymm8) (%_% ymm6) (%_% ymm14) *)
+  0xc4; 0x41; 0x5d; 0xd5; 0xd6;
+                           (* VPMULLW (%_% ymm10) (%_% ymm4) (%_% ymm14) *)
+  0xc5; 0xfd; 0xe5; 0xff;  (* VPMULHW (%_% ymm7) (%_% ymm0) (%_% ymm7) *)
+  0xc4; 0x41; 0x7d; 0xe5; 0xc9;
+                           (* VPMULHW (%_% ymm9) (%_% ymm0) (%_% ymm9) *)
+  0xc4; 0x41; 0x7d; 0xe5; 0xc0;
+                           (* VPMULHW (%_% ymm8) (%_% ymm0) (%_% ymm8) *)
+  0xc4; 0x41; 0x7d; 0xe5; 0xd2;
+                           (* VPMULHW (%_% ymm10) (%_% ymm0) (%_% ymm10) *)
+  0xc5; 0x5d; 0xe5; 0xda;  (* VPMULHW (%_% ymm11) (%_% ymm4) (%_% ymm2) *)
+  0xc5; 0x55; 0xe5; 0xe2;  (* VPMULHW (%_% ymm12) (%_% ymm5) (%_% ymm2) *)
+  0xc5; 0x4d; 0xe5; 0xeb;  (* VPMULHW (%_% ymm13) (%_% ymm6) (%_% ymm3) *)
+  0xc5; 0x5d; 0xe5; 0xf3;  (* VPMULHW (%_% ymm14) (%_% ymm4) (%_% ymm3) *)
+  0xc5; 0xa5; 0xf9; 0xff;  (* VPSUBW (%_% ymm7) (%_% ymm11) (%_% ymm7) *)
+  0xc4; 0x41; 0x1d; 0xf9; 0xc9;
+                           (* VPSUBW (%_% ymm9) (%_% ymm12) (%_% ymm9) *)
+  0xc4; 0x41; 0x3d; 0xf9; 0xc5;
+                           (* VPSUBW (%_% ymm8) (%_% ymm8) (%_% ymm13) *)
+  0xc4; 0x41; 0x0d; 0xf9; 0xd2;
+                           (* VPSUBW (%_% ymm10) (%_% ymm14) (%_% ymm10) *)
+  0xc5; 0xbd; 0xfd; 0xff;  (* VPADDW (%_% ymm7) (%_% ymm8) (%_% ymm7) *)
+  0xc4; 0x41; 0x2d; 0xfd; 0xc9;
+                           (* VPADDW (%_% ymm9) (%_% ymm10) (%_% ymm9) *)
+  0xc5; 0xfd; 0x7f; 0x7f; 0x40;
+                           (* VMOVDQA (Memop Word256 (%% (rdi,64))) (%_% ymm7) *)
+  0xc5; 0x7d; 0x7f; 0x4f; 0x60;
+                           (* VMOVDQA (Memop Word256 (%% (rdi,96))) (%_% ymm9) *)
+  0xc5; 0xfd; 0x6f; 0x96; 0x80; 0x00; 0x00; 0x00;
+                           (* VMOVDQA (%_% ymm2) (Memop Word256 (%% (rsi,128))) *)
+  0xc5; 0xfd; 0x6f; 0x9e; 0xa0; 0x00; 0x00; 0x00;
+                           (* VMOVDQA (%_% ymm3) (Memop Word256 (%% (rsi,160))) *)
+  0xc5; 0xfd; 0x6f; 0xa2; 0x80; 0x00; 0x00; 0x00;
+                           (* VMOVDQA (%_% ymm4) (Memop Word256 (%% (rdx,128))) *)
+  0xc5; 0xfd; 0x6f; 0xaa; 0xa0; 0x00; 0x00; 0x00;
+                           (* VMOVDQA (%_% ymm5) (Memop Word256 (%% (rdx,160))) *)
+  0xc5; 0xfd; 0x6f; 0x71; 0x40;
+                           (* VMOVDQA (%_% ymm6) (Memop Word256 (%% (rcx,64))) *)
+  0xc5; 0x75; 0xd5; 0xea;  (* VPMULLW (%_% ymm13) (%_% ymm1) (%_% ymm2) *)
+  0xc5; 0x75; 0xd5; 0xf3;  (* VPMULLW (%_% ymm14) (%_% ymm1) (%_% ymm3) *)
+  0xc4; 0xc1; 0x5d; 0xd5; 0xfd;
+                           (* VPMULLW (%_% ymm7) (%_% ymm4) (%_% ymm13) *)
+  0xc4; 0x41; 0x55; 0xd5; 0xcd;
+                           (* VPMULLW (%_% ymm9) (%_% ymm5) (%_% ymm13) *)
+  0xc4; 0x41; 0x4d; 0xd5; 0xc6;
+                           (* VPMULLW (%_% ymm8) (%_% ymm6) (%_% ymm14) *)
+  0xc4; 0x41; 0x5d; 0xd5; 0xd6;
+                           (* VPMULLW (%_% ymm10) (%_% ymm4) (%_% ymm14) *)
+  0xc5; 0xfd; 0xe5; 0xff;  (* VPMULHW (%_% ymm7) (%_% ymm0) (%_% ymm7) *)
+  0xc4; 0x41; 0x7d; 0xe5; 0xc9;
+                           (* VPMULHW (%_% ymm9) (%_% ymm0) (%_% ymm9) *)
+  0xc4; 0x41; 0x7d; 0xe5; 0xc0;
+                           (* VPMULHW (%_% ymm8) (%_% ymm0) (%_% ymm8) *)
+  0xc4; 0x41; 0x7d; 0xe5; 0xd2;
+                           (* VPMULHW (%_% ymm10) (%_% ymm0) (%_% ymm10) *)
+  0xc5; 0x5d; 0xe5; 0xda;  (* VPMULHW (%_% ymm11) (%_% ymm4) (%_% ymm2) *)
+  0xc5; 0x55; 0xe5; 0xe2;  (* VPMULHW (%_% ymm12) (%_% ymm5) (%_% ymm2) *)
+  0xc5; 0x4d; 0xe5; 0xeb;  (* VPMULHW (%_% ymm13) (%_% ymm6) (%_% ymm3) *)
+  0xc5; 0x5d; 0xe5; 0xf3;  (* VPMULHW (%_% ymm14) (%_% ymm4) (%_% ymm3) *)
+  0xc5; 0xa5; 0xf9; 0xff;  (* VPSUBW (%_% ymm7) (%_% ymm11) (%_% ymm7) *)
+  0xc4; 0x41; 0x1d; 0xf9; 0xc9;
+                           (* VPSUBW (%_% ymm9) (%_% ymm12) (%_% ymm9) *)
+  0xc4; 0x41; 0x15; 0xf9; 0xc0;
+                           (* VPSUBW (%_% ymm8) (%_% ymm13) (%_% ymm8) *)
+  0xc4; 0x41; 0x0d; 0xf9; 0xd2;
+                           (* VPSUBW (%_% ymm10) (%_% ymm14) (%_% ymm10) *)
+  0xc5; 0xbd; 0xfd; 0xff;  (* VPADDW (%_% ymm7) (%_% ymm8) (%_% ymm7) *)
+  0xc4; 0x41; 0x2d; 0xfd; 0xc9;
+                           (* VPADDW (%_% ymm9) (%_% ymm10) (%_% ymm9) *)
+  0xc5; 0xfd; 0x7f; 0xbf; 0x80; 0x00; 0x00; 0x00;
+                           (* VMOVDQA (Memop Word256 (%% (rdi,128))) (%_% ymm7) *)
+  0xc5; 0x7d; 0x7f; 0x8f; 0xa0; 0x00; 0x00; 0x00;
+                           (* VMOVDQA (Memop Word256 (%% (rdi,160))) (%_% ymm9) *)
+  0xc5; 0xfd; 0x6f; 0x96; 0xc0; 0x00; 0x00; 0x00;
+                           (* VMOVDQA (%_% ymm2) (Memop Word256 (%% (rsi,192))) *)
+  0xc5; 0xfd; 0x6f; 0x9e; 0xe0; 0x00; 0x00; 0x00;
+                           (* VMOVDQA (%_% ymm3) (Memop Word256 (%% (rsi,224))) *)
+  0xc5; 0xfd; 0x6f; 0xa2; 0xc0; 0x00; 0x00; 0x00;
+                           (* VMOVDQA (%_% ymm4) (Memop Word256 (%% (rdx,192))) *)
+  0xc5; 0xfd; 0x6f; 0xaa; 0xe0; 0x00; 0x00; 0x00;
+                           (* VMOVDQA (%_% ymm5) (Memop Word256 (%% (rdx,224))) *)
+  0xc5; 0xfd; 0x6f; 0x71; 0x60;
+                           (* VMOVDQA (%_% ymm6) (Memop Word256 (%% (rcx,96))) *)
+  0xc5; 0x75; 0xd5; 0xea;  (* VPMULLW (%_% ymm13) (%_% ymm1) (%_% ymm2) *)
+  0xc5; 0x75; 0xd5; 0xf3;  (* VPMULLW (%_% ymm14) (%_% ymm1) (%_% ymm3) *)
+  0xc4; 0xc1; 0x5d; 0xd5; 0xfd;
+                           (* VPMULLW (%_% ymm7) (%_% ymm4) (%_% ymm13) *)
+  0xc4; 0x41; 0x55; 0xd5; 0xcd;
+                           (* VPMULLW (%_% ymm9) (%_% ymm5) (%_% ymm13) *)
+  0xc4; 0x41; 0x4d; 0xd5; 0xc6;
+                           (* VPMULLW (%_% ymm8) (%_% ymm6) (%_% ymm14) *)
+  0xc4; 0x41; 0x5d; 0xd5; 0xd6;
+                           (* VPMULLW (%_% ymm10) (%_% ymm4) (%_% ymm14) *)
+  0xc5; 0xfd; 0xe5; 0xff;  (* VPMULHW (%_% ymm7) (%_% ymm0) (%_% ymm7) *)
+  0xc4; 0x41; 0x7d; 0xe5; 0xc9;
+                           (* VPMULHW (%_% ymm9) (%_% ymm0) (%_% ymm9) *)
+  0xc4; 0x41; 0x7d; 0xe5; 0xc0;
+                           (* VPMULHW (%_% ymm8) (%_% ymm0) (%_% ymm8) *)
+  0xc4; 0x41; 0x7d; 0xe5; 0xd2;
+                           (* VPMULHW (%_% ymm10) (%_% ymm0) (%_% ymm10) *)
+  0xc5; 0x5d; 0xe5; 0xda;  (* VPMULHW (%_% ymm11) (%_% ymm4) (%_% ymm2) *)
+  0xc5; 0x55; 0xe5; 0xe2;  (* VPMULHW (%_% ymm12) (%_% ymm5) (%_% ymm2) *)
+  0xc5; 0x4d; 0xe5; 0xeb;  (* VPMULHW (%_% ymm13) (%_% ymm6) (%_% ymm3) *)
+  0xc5; 0x5d; 0xe5; 0xf3;  (* VPMULHW (%_% ymm14) (%_% ymm4) (%_% ymm3) *)
+  0xc5; 0xa5; 0xf9; 0xff;  (* VPSUBW (%_% ymm7) (%_% ymm11) (%_% ymm7) *)
+  0xc4; 0x41; 0x1d; 0xf9; 0xc9;
+                           (* VPSUBW (%_% ymm9) (%_% ymm12) (%_% ymm9) *)
+  0xc4; 0x41; 0x3d; 0xf9; 0xc5;
+                           (* VPSUBW (%_% ymm8) (%_% ymm8) (%_% ymm13) *)
+  0xc4; 0x41; 0x0d; 0xf9; 0xd2;
+                           (* VPSUBW (%_% ymm10) (%_% ymm14) (%_% ymm10) *)
+  0xc5; 0xbd; 0xfd; 0xff;  (* VPADDW (%_% ymm7) (%_% ymm8) (%_% ymm7) *)
+  0xc4; 0x41; 0x2d; 0xfd; 0xc9;
+                           (* VPADDW (%_% ymm9) (%_% ymm10) (%_% ymm9) *)
+  0xc5; 0xfd; 0x7f; 0xbf; 0xc0; 0x00; 0x00; 0x00;
+                           (* VMOVDQA (Memop Word256 (%% (rdi,192))) (%_% ymm7) *)
+  0xc5; 0x7d; 0x7f; 0x8f; 0xe0; 0x00; 0x00; 0x00;
+                           (* VMOVDQA (Memop Word256 (%% (rdi,224))) (%_% ymm9) *)
+  0xc5; 0xfd; 0x6f; 0x96; 0x00; 0x01; 0x00; 0x00;
+                           (* VMOVDQA (%_% ymm2) (Memop Word256 (%% (rsi,256))) *)
+  0xc5; 0xfd; 0x6f; 0x9e; 0x20; 0x01; 0x00; 0x00;
+                           (* VMOVDQA (%_% ymm3) (Memop Word256 (%% (rsi,288))) *)
+  0xc5; 0xfd; 0x6f; 0xa2; 0x00; 0x01; 0x00; 0x00;
+                           (* VMOVDQA (%_% ymm4) (Memop Word256 (%% (rdx,256))) *)
+  0xc5; 0xfd; 0x6f; 0xaa; 0x20; 0x01; 0x00; 0x00;
+                           (* VMOVDQA (%_% ymm5) (Memop Word256 (%% (rdx,288))) *)
+  0xc5; 0xfd; 0x6f; 0xb1; 0x80; 0x00; 0x00; 0x00;
+                           (* VMOVDQA (%_% ymm6) (Memop Word256 (%% (rcx,128))) *)
+  0xc5; 0x75; 0xd5; 0xea;  (* VPMULLW (%_% ymm13) (%_% ymm1) (%_% ymm2) *)
+  0xc5; 0x75; 0xd5; 0xf3;  (* VPMULLW (%_% ymm14) (%_% ymm1) (%_% ymm3) *)
+  0xc4; 0xc1; 0x5d; 0xd5; 0xfd;
+                           (* VPMULLW (%_% ymm7) (%_% ymm4) (%_% ymm13) *)
+  0xc4; 0x41; 0x55; 0xd5; 0xcd;
+                           (* VPMULLW (%_% ymm9) (%_% ymm5) (%_% ymm13) *)
+  0xc4; 0x41; 0x4d; 0xd5; 0xc6;
+                           (* VPMULLW (%_% ymm8) (%_% ymm6) (%_% ymm14) *)
+  0xc4; 0x41; 0x5d; 0xd5; 0xd6;
+                           (* VPMULLW (%_% ymm10) (%_% ymm4) (%_% ymm14) *)
+  0xc5; 0xfd; 0xe5; 0xff;  (* VPMULHW (%_% ymm7) (%_% ymm0) (%_% ymm7) *)
+  0xc4; 0x41; 0x7d; 0xe5; 0xc9;
+                           (* VPMULHW (%_% ymm9) (%_% ymm0) (%_% ymm9) *)
+  0xc4; 0x41; 0x7d; 0xe5; 0xc0;
+                           (* VPMULHW (%_% ymm8) (%_% ymm0) (%_% ymm8) *)
+  0xc4; 0x41; 0x7d; 0xe5; 0xd2;
+                           (* VPMULHW (%_% ymm10) (%_% ymm0) (%_% ymm10) *)
+  0xc5; 0x5d; 0xe5; 0xda;  (* VPMULHW (%_% ymm11) (%_% ymm4) (%_% ymm2) *)
+  0xc5; 0x55; 0xe5; 0xe2;  (* VPMULHW (%_% ymm12) (%_% ymm5) (%_% ymm2) *)
+  0xc5; 0x4d; 0xe5; 0xeb;  (* VPMULHW (%_% ymm13) (%_% ymm6) (%_% ymm3) *)
+  0xc5; 0x5d; 0xe5; 0xf3;  (* VPMULHW (%_% ymm14) (%_% ymm4) (%_% ymm3) *)
+  0xc5; 0xa5; 0xf9; 0xff;  (* VPSUBW (%_% ymm7) (%_% ymm11) (%_% ymm7) *)
+  0xc4; 0x41; 0x1d; 0xf9; 0xc9;
+                           (* VPSUBW (%_% ymm9) (%_% ymm12) (%_% ymm9) *)
+  0xc4; 0x41; 0x15; 0xf9; 0xc0;
+                           (* VPSUBW (%_% ymm8) (%_% ymm13) (%_% ymm8) *)
+  0xc4; 0x41; 0x0d; 0xf9; 0xd2;
+                           (* VPSUBW (%_% ymm10) (%_% ymm14) (%_% ymm10) *)
+  0xc5; 0xbd; 0xfd; 0xff;  (* VPADDW (%_% ymm7) (%_% ymm8) (%_% ymm7) *)
+  0xc4; 0x41; 0x2d; 0xfd; 0xc9;
+                           (* VPADDW (%_% ymm9) (%_% ymm10) (%_% ymm9) *)
+  0xc5; 0xfd; 0x7f; 0xbf; 0x00; 0x01; 0x00; 0x00;
+                           (* VMOVDQA (Memop Word256 (%% (rdi,256))) (%_% ymm7) *)
+  0xc5; 0x7d; 0x7f; 0x8f; 0x20; 0x01; 0x00; 0x00;
+                           (* VMOVDQA (Memop Word256 (%% (rdi,288))) (%_% ymm9) *)
+  0xc5; 0xfd; 0x6f; 0x96; 0x40; 0x01; 0x00; 0x00;
+                           (* VMOVDQA (%_% ymm2) (Memop Word256 (%% (rsi,320))) *)
+  0xc5; 0xfd; 0x6f; 0x9e; 0x60; 0x01; 0x00; 0x00;
+                           (* VMOVDQA (%_% ymm3) (Memop Word256 (%% (rsi,352))) *)
+  0xc5; 0xfd; 0x6f; 0xa2; 0x40; 0x01; 0x00; 0x00;
+                           (* VMOVDQA (%_% ymm4) (Memop Word256 (%% (rdx,320))) *)
+  0xc5; 0xfd; 0x6f; 0xaa; 0x60; 0x01; 0x00; 0x00;
+                           (* VMOVDQA (%_% ymm5) (Memop Word256 (%% (rdx,352))) *)
+  0xc5; 0xfd; 0x6f; 0xb1; 0xa0; 0x00; 0x00; 0x00;
+                           (* VMOVDQA (%_% ymm6) (Memop Word256 (%% (rcx,160))) *)
+  0xc5; 0x75; 0xd5; 0xea;  (* VPMULLW (%_% ymm13) (%_% ymm1) (%_% ymm2) *)
+  0xc5; 0x75; 0xd5; 0xf3;  (* VPMULLW (%_% ymm14) (%_% ymm1) (%_% ymm3) *)
+  0xc4; 0xc1; 0x5d; 0xd5; 0xfd;
+                           (* VPMULLW (%_% ymm7) (%_% ymm4) (%_% ymm13) *)
+  0xc4; 0x41; 0x55; 0xd5; 0xcd;
+                           (* VPMULLW (%_% ymm9) (%_% ymm5) (%_% ymm13) *)
+  0xc4; 0x41; 0x4d; 0xd5; 0xc6;
+                           (* VPMULLW (%_% ymm8) (%_% ymm6) (%_% ymm14) *)
+  0xc4; 0x41; 0x5d; 0xd5; 0xd6;
+                           (* VPMULLW (%_% ymm10) (%_% ymm4) (%_% ymm14) *)
+  0xc5; 0xfd; 0xe5; 0xff;  (* VPMULHW (%_% ymm7) (%_% ymm0) (%_% ymm7) *)
+  0xc4; 0x41; 0x7d; 0xe5; 0xc9;
+                           (* VPMULHW (%_% ymm9) (%_% ymm0) (%_% ymm9) *)
+  0xc4; 0x41; 0x7d; 0xe5; 0xc0;
+                           (* VPMULHW (%_% ymm8) (%_% ymm0) (%_% ymm8) *)
+  0xc4; 0x41; 0x7d; 0xe5; 0xd2;
+                           (* VPMULHW (%_% ymm10) (%_% ymm0) (%_% ymm10) *)
+  0xc5; 0x5d; 0xe5; 0xda;  (* VPMULHW (%_% ymm11) (%_% ymm4) (%_% ymm2) *)
+  0xc5; 0x55; 0xe5; 0xe2;  (* VPMULHW (%_% ymm12) (%_% ymm5) (%_% ymm2) *)
+  0xc5; 0x4d; 0xe5; 0xeb;  (* VPMULHW (%_% ymm13) (%_% ymm6) (%_% ymm3) *)
+  0xc5; 0x5d; 0xe5; 0xf3;  (* VPMULHW (%_% ymm14) (%_% ymm4) (%_% ymm3) *)
+  0xc5; 0xa5; 0xf9; 0xff;  (* VPSUBW (%_% ymm7) (%_% ymm11) (%_% ymm7) *)
+  0xc4; 0x41; 0x1d; 0xf9; 0xc9;
+                           (* VPSUBW (%_% ymm9) (%_% ymm12) (%_% ymm9) *)
+  0xc4; 0x41; 0x3d; 0xf9; 0xc5;
+                           (* VPSUBW (%_% ymm8) (%_% ymm8) (%_% ymm13) *)
+  0xc4; 0x41; 0x0d; 0xf9; 0xd2;
+                           (* VPSUBW (%_% ymm10) (%_% ymm14) (%_% ymm10) *)
+  0xc5; 0xbd; 0xfd; 0xff;  (* VPADDW (%_% ymm7) (%_% ymm8) (%_% ymm7) *)
+  0xc4; 0x41; 0x2d; 0xfd; 0xc9;
+                           (* VPADDW (%_% ymm9) (%_% ymm10) (%_% ymm9) *)
+  0xc5; 0xfd; 0x7f; 0xbf; 0x40; 0x01; 0x00; 0x00;
+                           (* VMOVDQA (Memop Word256 (%% (rdi,320))) (%_% ymm7) *)
+  0xc5; 0x7d; 0x7f; 0x8f; 0x60; 0x01; 0x00; 0x00;
+                           (* VMOVDQA (Memop Word256 (%% (rdi,352))) (%_% ymm9) *)
+  0xc5; 0xfd; 0x6f; 0x96; 0x80; 0x01; 0x00; 0x00;
+                           (* VMOVDQA (%_% ymm2) (Memop Word256 (%% (rsi,384))) *)
+  0xc5; 0xfd; 0x6f; 0x9e; 0xa0; 0x01; 0x00; 0x00;
+                           (* VMOVDQA (%_% ymm3) (Memop Word256 (%% (rsi,416))) *)
+  0xc5; 0xfd; 0x6f; 0xa2; 0x80; 0x01; 0x00; 0x00;
+                           (* VMOVDQA (%_% ymm4) (Memop Word256 (%% (rdx,384))) *)
+  0xc5; 0xfd; 0x6f; 0xaa; 0xa0; 0x01; 0x00; 0x00;
+                           (* VMOVDQA (%_% ymm5) (Memop Word256 (%% (rdx,416))) *)
+  0xc5; 0xfd; 0x6f; 0xb1; 0xc0; 0x00; 0x00; 0x00;
+                           (* VMOVDQA (%_% ymm6) (Memop Word256 (%% (rcx,192))) *)
+  0xc5; 0x75; 0xd5; 0xea;  (* VPMULLW (%_% ymm13) (%_% ymm1) (%_% ymm2) *)
+  0xc5; 0x75; 0xd5; 0xf3;  (* VPMULLW (%_% ymm14) (%_% ymm1) (%_% ymm3) *)
+  0xc4; 0xc1; 0x5d; 0xd5; 0xfd;
+                           (* VPMULLW (%_% ymm7) (%_% ymm4) (%_% ymm13) *)
+  0xc4; 0x41; 0x55; 0xd5; 0xcd;
+                           (* VPMULLW (%_% ymm9) (%_% ymm5) (%_% ymm13) *)
+  0xc4; 0x41; 0x4d; 0xd5; 0xc6;
+                           (* VPMULLW (%_% ymm8) (%_% ymm6) (%_% ymm14) *)
+  0xc4; 0x41; 0x5d; 0xd5; 0xd6;
+                           (* VPMULLW (%_% ymm10) (%_% ymm4) (%_% ymm14) *)
+  0xc5; 0xfd; 0xe5; 0xff;  (* VPMULHW (%_% ymm7) (%_% ymm0) (%_% ymm7) *)
+  0xc4; 0x41; 0x7d; 0xe5; 0xc9;
+                           (* VPMULHW (%_% ymm9) (%_% ymm0) (%_% ymm9) *)
+  0xc4; 0x41; 0x7d; 0xe5; 0xc0;
+                           (* VPMULHW (%_% ymm8) (%_% ymm0) (%_% ymm8) *)
+  0xc4; 0x41; 0x7d; 0xe5; 0xd2;
+                           (* VPMULHW (%_% ymm10) (%_% ymm0) (%_% ymm10) *)
+  0xc5; 0x5d; 0xe5; 0xda;  (* VPMULHW (%_% ymm11) (%_% ymm4) (%_% ymm2) *)
+  0xc5; 0x55; 0xe5; 0xe2;  (* VPMULHW (%_% ymm12) (%_% ymm5) (%_% ymm2) *)
+  0xc5; 0x4d; 0xe5; 0xeb;  (* VPMULHW (%_% ymm13) (%_% ymm6) (%_% ymm3) *)
+  0xc5; 0x5d; 0xe5; 0xf3;  (* VPMULHW (%_% ymm14) (%_% ymm4) (%_% ymm3) *)
+  0xc5; 0xa5; 0xf9; 0xff;  (* VPSUBW (%_% ymm7) (%_% ymm11) (%_% ymm7) *)
+  0xc4; 0x41; 0x1d; 0xf9; 0xc9;
+                           (* VPSUBW (%_% ymm9) (%_% ymm12) (%_% ymm9) *)
+  0xc4; 0x41; 0x15; 0xf9; 0xc0;
+                           (* VPSUBW (%_% ymm8) (%_% ymm13) (%_% ymm8) *)
+  0xc4; 0x41; 0x0d; 0xf9; 0xd2;
+                           (* VPSUBW (%_% ymm10) (%_% ymm14) (%_% ymm10) *)
+  0xc5; 0xbd; 0xfd; 0xff;  (* VPADDW (%_% ymm7) (%_% ymm8) (%_% ymm7) *)
+  0xc4; 0x41; 0x2d; 0xfd; 0xc9;
+                           (* VPADDW (%_% ymm9) (%_% ymm10) (%_% ymm9) *)
+  0xc5; 0xfd; 0x7f; 0xbf; 0x80; 0x01; 0x00; 0x00;
+                           (* VMOVDQA (Memop Word256 (%% (rdi,384))) (%_% ymm7) *)
+  0xc5; 0x7d; 0x7f; 0x8f; 0xa0; 0x01; 0x00; 0x00;
+                           (* VMOVDQA (Memop Word256 (%% (rdi,416))) (%_% ymm9) *)
+  0xc5; 0xfd; 0x6f; 0x96; 0xc0; 0x01; 0x00; 0x00;
+                           (* VMOVDQA (%_% ymm2) (Memop Word256 (%% (rsi,448))) *)
+  0xc5; 0xfd; 0x6f; 0x9e; 0xe0; 0x01; 0x00; 0x00;
+                           (* VMOVDQA (%_% ymm3) (Memop Word256 (%% (rsi,480))) *)
+  0xc5; 0xfd; 0x6f; 0xa2; 0xc0; 0x01; 0x00; 0x00;
+                           (* VMOVDQA (%_% ymm4) (Memop Word256 (%% (rdx,448))) *)
+  0xc5; 0xfd; 0x6f; 0xaa; 0xe0; 0x01; 0x00; 0x00;
+                           (* VMOVDQA (%_% ymm5) (Memop Word256 (%% (rdx,480))) *)
+  0xc5; 0xfd; 0x6f; 0xb1; 0xe0; 0x00; 0x00; 0x00;
+                           (* VMOVDQA (%_% ymm6) (Memop Word256 (%% (rcx,224))) *)
+  0xc5; 0x75; 0xd5; 0xea;  (* VPMULLW (%_% ymm13) (%_% ymm1) (%_% ymm2) *)
+  0xc5; 0x75; 0xd5; 0xf3;  (* VPMULLW (%_% ymm14) (%_% ymm1) (%_% ymm3) *)
+  0xc4; 0xc1; 0x5d; 0xd5; 0xfd;
+                           (* VPMULLW (%_% ymm7) (%_% ymm4) (%_% ymm13) *)
+  0xc4; 0x41; 0x55; 0xd5; 0xcd;
+                           (* VPMULLW (%_% ymm9) (%_% ymm5) (%_% ymm13) *)
+  0xc4; 0x41; 0x4d; 0xd5; 0xc6;
+                           (* VPMULLW (%_% ymm8) (%_% ymm6) (%_% ymm14) *)
+  0xc4; 0x41; 0x5d; 0xd5; 0xd6;
+                           (* VPMULLW (%_% ymm10) (%_% ymm4) (%_% ymm14) *)
+  0xc5; 0xfd; 0xe5; 0xff;  (* VPMULHW (%_% ymm7) (%_% ymm0) (%_% ymm7) *)
+  0xc4; 0x41; 0x7d; 0xe5; 0xc9;
+                           (* VPMULHW (%_% ymm9) (%_% ymm0) (%_% ymm9) *)
+  0xc4; 0x41; 0x7d; 0xe5; 0xc0;
+                           (* VPMULHW (%_% ymm8) (%_% ymm0) (%_% ymm8) *)
+  0xc4; 0x41; 0x7d; 0xe5; 0xd2;
+                           (* VPMULHW (%_% ymm10) (%_% ymm0) (%_% ymm10) *)
+  0xc5; 0x5d; 0xe5; 0xda;  (* VPMULHW (%_% ymm11) (%_% ymm4) (%_% ymm2) *)
+  0xc5; 0x55; 0xe5; 0xe2;  (* VPMULHW (%_% ymm12) (%_% ymm5) (%_% ymm2) *)
+  0xc5; 0x4d; 0xe5; 0xeb;  (* VPMULHW (%_% ymm13) (%_% ymm6) (%_% ymm3) *)
+  0xc5; 0x5d; 0xe5; 0xf3;  (* VPMULHW (%_% ymm14) (%_% ymm4) (%_% ymm3) *)
+  0xc5; 0xa5; 0xf9; 0xff;  (* VPSUBW (%_% ymm7) (%_% ymm11) (%_% ymm7) *)
+  0xc4; 0x41; 0x1d; 0xf9; 0xc9;
+                           (* VPSUBW (%_% ymm9) (%_% ymm12) (%_% ymm9) *)
+  0xc4; 0x41; 0x3d; 0xf9; 0xc5;
+                           (* VPSUBW (%_% ymm8) (%_% ymm8) (%_% ymm13) *)
+  0xc4; 0x41; 0x0d; 0xf9; 0xd2;
+                           (* VPSUBW (%_% ymm10) (%_% ymm14) (%_% ymm10) *)
+  0xc5; 0xbd; 0xfd; 0xff;  (* VPADDW (%_% ymm7) (%_% ymm8) (%_% ymm7) *)
+  0xc4; 0x41; 0x2d; 0xfd; 0xc9;
+                           (* VPADDW (%_% ymm9) (%_% ymm10) (%_% ymm9) *)
+  0xc5; 0xfd; 0x7f; 0xbf; 0xc0; 0x01; 0x00; 0x00;
+                           (* VMOVDQA (Memop Word256 (%% (rdi,448))) (%_% ymm7) *)
+  0xc5; 0x7d; 0x7f; 0x8f; 0xe0; 0x01; 0x00; 0x00;
+                           (* VMOVDQA (Memop Word256 (%% (rdi,480))) (%_% ymm9) *)
+  0xc5; 0xfd; 0x6f; 0x96; 0x00; 0x02; 0x00; 0x00;
+                           (* VMOVDQA (%_% ymm2) (Memop Word256 (%% (rsi,512))) *)
+  0xc5; 0xfd; 0x6f; 0x9e; 0x20; 0x02; 0x00; 0x00;
+                           (* VMOVDQA (%_% ymm3) (Memop Word256 (%% (rsi,544))) *)
+  0xc5; 0xfd; 0x6f; 0xa2; 0x00; 0x02; 0x00; 0x00;
+                           (* VMOVDQA (%_% ymm4) (Memop Word256 (%% (rdx,512))) *)
+  0xc5; 0xfd; 0x6f; 0xaa; 0x20; 0x02; 0x00; 0x00;
+                           (* VMOVDQA (%_% ymm5) (Memop Word256 (%% (rdx,544))) *)
+  0xc5; 0xfd; 0x6f; 0xb1; 0x00; 0x01; 0x00; 0x00;
+                           (* VMOVDQA (%_% ymm6) (Memop Word256 (%% (rcx,256))) *)
+  0xc5; 0x75; 0xd5; 0xea;  (* VPMULLW (%_% ymm13) (%_% ymm1) (%_% ymm2) *)
+  0xc5; 0x75; 0xd5; 0xf3;  (* VPMULLW (%_% ymm14) (%_% ymm1) (%_% ymm3) *)
+  0xc4; 0xc1; 0x5d; 0xd5; 0xfd;
+                           (* VPMULLW (%_% ymm7) (%_% ymm4) (%_% ymm13) *)
+  0xc4; 0x41; 0x55; 0xd5; 0xcd;
+                           (* VPMULLW (%_% ymm9) (%_% ymm5) (%_% ymm13) *)
+  0xc4; 0x41; 0x4d; 0xd5; 0xc6;
+                           (* VPMULLW (%_% ymm8) (%_% ymm6) (%_% ymm14) *)
+  0xc4; 0x41; 0x5d; 0xd5; 0xd6;
+                           (* VPMULLW (%_% ymm10) (%_% ymm4) (%_% ymm14) *)
+  0xc5; 0xfd; 0xe5; 0xff;  (* VPMULHW (%_% ymm7) (%_% ymm0) (%_% ymm7) *)
+  0xc4; 0x41; 0x7d; 0xe5; 0xc9;
+                           (* VPMULHW (%_% ymm9) (%_% ymm0) (%_% ymm9) *)
+  0xc4; 0x41; 0x7d; 0xe5; 0xc0;
+                           (* VPMULHW (%_% ymm8) (%_% ymm0) (%_% ymm8) *)
+  0xc4; 0x41; 0x7d; 0xe5; 0xd2;
+                           (* VPMULHW (%_% ymm10) (%_% ymm0) (%_% ymm10) *)
+  0xc5; 0x5d; 0xe5; 0xda;  (* VPMULHW (%_% ymm11) (%_% ymm4) (%_% ymm2) *)
+  0xc5; 0x55; 0xe5; 0xe2;  (* VPMULHW (%_% ymm12) (%_% ymm5) (%_% ymm2) *)
+  0xc5; 0x4d; 0xe5; 0xeb;  (* VPMULHW (%_% ymm13) (%_% ymm6) (%_% ymm3) *)
+  0xc5; 0x5d; 0xe5; 0xf3;  (* VPMULHW (%_% ymm14) (%_% ymm4) (%_% ymm3) *)
+  0xc5; 0xa5; 0xf9; 0xff;  (* VPSUBW (%_% ymm7) (%_% ymm11) (%_% ymm7) *)
+  0xc4; 0x41; 0x1d; 0xf9; 0xc9;
+                           (* VPSUBW (%_% ymm9) (%_% ymm12) (%_% ymm9) *)
+  0xc4; 0x41; 0x15; 0xf9; 0xc0;
+                           (* VPSUBW (%_% ymm8) (%_% ymm13) (%_% ymm8) *)
+  0xc4; 0x41; 0x0d; 0xf9; 0xd2;
+                           (* VPSUBW (%_% ymm10) (%_% ymm14) (%_% ymm10) *)
+  0xc5; 0xbd; 0xfd; 0xff;  (* VPADDW (%_% ymm7) (%_% ymm8) (%_% ymm7) *)
+  0xc4; 0x41; 0x2d; 0xfd; 0xc9;
+                           (* VPADDW (%_% ymm9) (%_% ymm10) (%_% ymm9) *)
+  0xc5; 0x7d; 0x6f; 0x07;  (* VMOVDQA (%_% ymm8) (Memop Word256 (%% (rdi,0))) *)
+  0xc5; 0x7d; 0x6f; 0x57; 0x20;
+                           (* VMOVDQA (%_% ymm10) (Memop Word256 (%% (rdi,32))) *)
+  0xc5; 0xbd; 0xfd; 0xff;  (* VPADDW (%_% ymm7) (%_% ymm8) (%_% ymm7) *)
+  0xc4; 0x41; 0x2d; 0xfd; 0xc9;
+                           (* VPADDW (%_% ymm9) (%_% ymm10) (%_% ymm9) *)
+  0xc5; 0xfd; 0x7f; 0x3f;  (* VMOVDQA (Memop Word256 (%% (rdi,0))) (%_% ymm7) *)
+  0xc5; 0x7d; 0x7f; 0x4f; 0x20;
+                           (* VMOVDQA (Memop Word256 (%% (rdi,32))) (%_% ymm9) *)
+  0xc5; 0xfd; 0x6f; 0x96; 0x40; 0x02; 0x00; 0x00;
+                           (* VMOVDQA (%_% ymm2) (Memop Word256 (%% (rsi,576))) *)
+  0xc5; 0xfd; 0x6f; 0x9e; 0x60; 0x02; 0x00; 0x00;
+                           (* VMOVDQA (%_% ymm3) (Memop Word256 (%% (rsi,608))) *)
+  0xc5; 0xfd; 0x6f; 0xa2; 0x40; 0x02; 0x00; 0x00;
+                           (* VMOVDQA (%_% ymm4) (Memop Word256 (%% (rdx,576))) *)
+  0xc5; 0xfd; 0x6f; 0xaa; 0x60; 0x02; 0x00; 0x00;
+                           (* VMOVDQA (%_% ymm5) (Memop Word256 (%% (rdx,608))) *)
+  0xc5; 0xfd; 0x6f; 0xb1; 0x20; 0x01; 0x00; 0x00;
+                           (* VMOVDQA (%_% ymm6) (Memop Word256 (%% (rcx,288))) *)
+  0xc5; 0x75; 0xd5; 0xea;  (* VPMULLW (%_% ymm13) (%_% ymm1) (%_% ymm2) *)
+  0xc5; 0x75; 0xd5; 0xf3;  (* VPMULLW (%_% ymm14) (%_% ymm1) (%_% ymm3) *)
+  0xc4; 0xc1; 0x5d; 0xd5; 0xfd;
+                           (* VPMULLW (%_% ymm7) (%_% ymm4) (%_% ymm13) *)
+  0xc4; 0x41; 0x55; 0xd5; 0xcd;
+                           (* VPMULLW (%_% ymm9) (%_% ymm5) (%_% ymm13) *)
+  0xc4; 0x41; 0x4d; 0xd5; 0xc6;
+                           (* VPMULLW (%_% ymm8) (%_% ymm6) (%_% ymm14) *)
+  0xc4; 0x41; 0x5d; 0xd5; 0xd6;
+                           (* VPMULLW (%_% ymm10) (%_% ymm4) (%_% ymm14) *)
+  0xc5; 0xfd; 0xe5; 0xff;  (* VPMULHW (%_% ymm7) (%_% ymm0) (%_% ymm7) *)
+  0xc4; 0x41; 0x7d; 0xe5; 0xc9;
+                           (* VPMULHW (%_% ymm9) (%_% ymm0) (%_% ymm9) *)
+  0xc4; 0x41; 0x7d; 0xe5; 0xc0;
+                           (* VPMULHW (%_% ymm8) (%_% ymm0) (%_% ymm8) *)
+  0xc4; 0x41; 0x7d; 0xe5; 0xd2;
+                           (* VPMULHW (%_% ymm10) (%_% ymm0) (%_% ymm10) *)
+  0xc5; 0x5d; 0xe5; 0xda;  (* VPMULHW (%_% ymm11) (%_% ymm4) (%_% ymm2) *)
+  0xc5; 0x55; 0xe5; 0xe2;  (* VPMULHW (%_% ymm12) (%_% ymm5) (%_% ymm2) *)
+  0xc5; 0x4d; 0xe5; 0xeb;  (* VPMULHW (%_% ymm13) (%_% ymm6) (%_% ymm3) *)
+  0xc5; 0x5d; 0xe5; 0xf3;  (* VPMULHW (%_% ymm14) (%_% ymm4) (%_% ymm3) *)
+  0xc5; 0xa5; 0xf9; 0xff;  (* VPSUBW (%_% ymm7) (%_% ymm11) (%_% ymm7) *)
+  0xc4; 0x41; 0x1d; 0xf9; 0xc9;
+                           (* VPSUBW (%_% ymm9) (%_% ymm12) (%_% ymm9) *)
+  0xc4; 0x41; 0x3d; 0xf9; 0xc5;
+                           (* VPSUBW (%_% ymm8) (%_% ymm8) (%_% ymm13) *)
+  0xc4; 0x41; 0x0d; 0xf9; 0xd2;
+                           (* VPSUBW (%_% ymm10) (%_% ymm14) (%_% ymm10) *)
+  0xc5; 0xbd; 0xfd; 0xff;  (* VPADDW (%_% ymm7) (%_% ymm8) (%_% ymm7) *)
+  0xc4; 0x41; 0x2d; 0xfd; 0xc9;
+                           (* VPADDW (%_% ymm9) (%_% ymm10) (%_% ymm9) *)
+  0xc5; 0x7d; 0x6f; 0x47; 0x40;
+                           (* VMOVDQA (%_% ymm8) (Memop Word256 (%% (rdi,64))) *)
+  0xc5; 0x7d; 0x6f; 0x57; 0x60;
+                           (* VMOVDQA (%_% ymm10) (Memop Word256 (%% (rdi,96))) *)
+  0xc5; 0xbd; 0xfd; 0xff;  (* VPADDW (%_% ymm7) (%_% ymm8) (%_% ymm7) *)
+  0xc4; 0x41; 0x2d; 0xfd; 0xc9;
+                           (* VPADDW (%_% ymm9) (%_% ymm10) (%_% ymm9) *)
+  0xc5; 0xfd; 0x7f; 0x7f; 0x40;
+                           (* VMOVDQA (Memop Word256 (%% (rdi,64))) (%_% ymm7) *)
+  0xc5; 0x7d; 0x7f; 0x4f; 0x60;
+                           (* VMOVDQA (Memop Word256 (%% (rdi,96))) (%_% ymm9) *)
+  0xc5; 0xfd; 0x6f; 0x96; 0x80; 0x02; 0x00; 0x00;
+                           (* VMOVDQA (%_% ymm2) (Memop Word256 (%% (rsi,640))) *)
+  0xc5; 0xfd; 0x6f; 0x9e; 0xa0; 0x02; 0x00; 0x00;
+                           (* VMOVDQA (%_% ymm3) (Memop Word256 (%% (rsi,672))) *)
+  0xc5; 0xfd; 0x6f; 0xa2; 0x80; 0x02; 0x00; 0x00;
+                           (* VMOVDQA (%_% ymm4) (Memop Word256 (%% (rdx,640))) *)
+  0xc5; 0xfd; 0x6f; 0xaa; 0xa0; 0x02; 0x00; 0x00;
+                           (* VMOVDQA (%_% ymm5) (Memop Word256 (%% (rdx,672))) *)
+  0xc5; 0xfd; 0x6f; 0xb1; 0x40; 0x01; 0x00; 0x00;
+                           (* VMOVDQA (%_% ymm6) (Memop Word256 (%% (rcx,320))) *)
+  0xc5; 0x75; 0xd5; 0xea;  (* VPMULLW (%_% ymm13) (%_% ymm1) (%_% ymm2) *)
+  0xc5; 0x75; 0xd5; 0xf3;  (* VPMULLW (%_% ymm14) (%_% ymm1) (%_% ymm3) *)
+  0xc4; 0xc1; 0x5d; 0xd5; 0xfd;
+                           (* VPMULLW (%_% ymm7) (%_% ymm4) (%_% ymm13) *)
+  0xc4; 0x41; 0x55; 0xd5; 0xcd;
+                           (* VPMULLW (%_% ymm9) (%_% ymm5) (%_% ymm13) *)
+  0xc4; 0x41; 0x4d; 0xd5; 0xc6;
+                           (* VPMULLW (%_% ymm8) (%_% ymm6) (%_% ymm14) *)
+  0xc4; 0x41; 0x5d; 0xd5; 0xd6;
+                           (* VPMULLW (%_% ymm10) (%_% ymm4) (%_% ymm14) *)
+  0xc5; 0xfd; 0xe5; 0xff;  (* VPMULHW (%_% ymm7) (%_% ymm0) (%_% ymm7) *)
+  0xc4; 0x41; 0x7d; 0xe5; 0xc9;
+                           (* VPMULHW (%_% ymm9) (%_% ymm0) (%_% ymm9) *)
+  0xc4; 0x41; 0x7d; 0xe5; 0xc0;
+                           (* VPMULHW (%_% ymm8) (%_% ymm0) (%_% ymm8) *)
+  0xc4; 0x41; 0x7d; 0xe5; 0xd2;
+                           (* VPMULHW (%_% ymm10) (%_% ymm0) (%_% ymm10) *)
+  0xc5; 0x5d; 0xe5; 0xda;  (* VPMULHW (%_% ymm11) (%_% ymm4) (%_% ymm2) *)
+  0xc5; 0x55; 0xe5; 0xe2;  (* VPMULHW (%_% ymm12) (%_% ymm5) (%_% ymm2) *)
+  0xc5; 0x4d; 0xe5; 0xeb;  (* VPMULHW (%_% ymm13) (%_% ymm6) (%_% ymm3) *)
+  0xc5; 0x5d; 0xe5; 0xf3;  (* VPMULHW (%_% ymm14) (%_% ymm4) (%_% ymm3) *)
+  0xc5; 0xa5; 0xf9; 0xff;  (* VPSUBW (%_% ymm7) (%_% ymm11) (%_% ymm7) *)
+  0xc4; 0x41; 0x1d; 0xf9; 0xc9;
+                           (* VPSUBW (%_% ymm9) (%_% ymm12) (%_% ymm9) *)
+  0xc4; 0x41; 0x15; 0xf9; 0xc0;
+                           (* VPSUBW (%_% ymm8) (%_% ymm13) (%_% ymm8) *)
+  0xc4; 0x41; 0x0d; 0xf9; 0xd2;
+                           (* VPSUBW (%_% ymm10) (%_% ymm14) (%_% ymm10) *)
+  0xc5; 0xbd; 0xfd; 0xff;  (* VPADDW (%_% ymm7) (%_% ymm8) (%_% ymm7) *)
+  0xc4; 0x41; 0x2d; 0xfd; 0xc9;
+                           (* VPADDW (%_% ymm9) (%_% ymm10) (%_% ymm9) *)
+  0xc5; 0x7d; 0x6f; 0x87; 0x80; 0x00; 0x00; 0x00;
+                           (* VMOVDQA (%_% ymm8) (Memop Word256 (%% (rdi,128))) *)
+  0xc5; 0x7d; 0x6f; 0x97; 0xa0; 0x00; 0x00; 0x00;
+                           (* VMOVDQA (%_% ymm10) (Memop Word256 (%% (rdi,160))) *)
+  0xc5; 0xbd; 0xfd; 0xff;  (* VPADDW (%_% ymm7) (%_% ymm8) (%_% ymm7) *)
+  0xc4; 0x41; 0x2d; 0xfd; 0xc9;
+                           (* VPADDW (%_% ymm9) (%_% ymm10) (%_% ymm9) *)
+  0xc5; 0xfd; 0x7f; 0xbf; 0x80; 0x00; 0x00; 0x00;
+                           (* VMOVDQA (Memop Word256 (%% (rdi,128))) (%_% ymm7) *)
+  0xc5; 0x7d; 0x7f; 0x8f; 0xa0; 0x00; 0x00; 0x00;
+                           (* VMOVDQA (Memop Word256 (%% (rdi,160))) (%_% ymm9) *)
+  0xc5; 0xfd; 0x6f; 0x96; 0xc0; 0x02; 0x00; 0x00;
+                           (* VMOVDQA (%_% ymm2) (Memop Word256 (%% (rsi,704))) *)
+  0xc5; 0xfd; 0x6f; 0x9e; 0xe0; 0x02; 0x00; 0x00;
+                           (* VMOVDQA (%_% ymm3) (Memop Word256 (%% (rsi,736))) *)
+  0xc5; 0xfd; 0x6f; 0xa2; 0xc0; 0x02; 0x00; 0x00;
+                           (* VMOVDQA (%_% ymm4) (Memop Word256 (%% (rdx,704))) *)
+  0xc5; 0xfd; 0x6f; 0xaa; 0xe0; 0x02; 0x00; 0x00;
+                           (* VMOVDQA (%_% ymm5) (Memop Word256 (%% (rdx,736))) *)
+  0xc5; 0xfd; 0x6f; 0xb1; 0x60; 0x01; 0x00; 0x00;
+                           (* VMOVDQA (%_% ymm6) (Memop Word256 (%% (rcx,352))) *)
+  0xc5; 0x75; 0xd5; 0xea;  (* VPMULLW (%_% ymm13) (%_% ymm1) (%_% ymm2) *)
+  0xc5; 0x75; 0xd5; 0xf3;  (* VPMULLW (%_% ymm14) (%_% ymm1) (%_% ymm3) *)
+  0xc4; 0xc1; 0x5d; 0xd5; 0xfd;
+                           (* VPMULLW (%_% ymm7) (%_% ymm4) (%_% ymm13) *)
+  0xc4; 0x41; 0x55; 0xd5; 0xcd;
+                           (* VPMULLW (%_% ymm9) (%_% ymm5) (%_% ymm13) *)
+  0xc4; 0x41; 0x4d; 0xd5; 0xc6;
+                           (* VPMULLW (%_% ymm8) (%_% ymm6) (%_% ymm14) *)
+  0xc4; 0x41; 0x5d; 0xd5; 0xd6;
+                           (* VPMULLW (%_% ymm10) (%_% ymm4) (%_% ymm14) *)
+  0xc5; 0xfd; 0xe5; 0xff;  (* VPMULHW (%_% ymm7) (%_% ymm0) (%_% ymm7) *)
+  0xc4; 0x41; 0x7d; 0xe5; 0xc9;
+                           (* VPMULHW (%_% ymm9) (%_% ymm0) (%_% ymm9) *)
+  0xc4; 0x41; 0x7d; 0xe5; 0xc0;
+                           (* VPMULHW (%_% ymm8) (%_% ymm0) (%_% ymm8) *)
+  0xc4; 0x41; 0x7d; 0xe5; 0xd2;
+                           (* VPMULHW (%_% ymm10) (%_% ymm0) (%_% ymm10) *)
+  0xc5; 0x5d; 0xe5; 0xda;  (* VPMULHW (%_% ymm11) (%_% ymm4) (%_% ymm2) *)
+  0xc5; 0x55; 0xe5; 0xe2;  (* VPMULHW (%_% ymm12) (%_% ymm5) (%_% ymm2) *)
+  0xc5; 0x4d; 0xe5; 0xeb;  (* VPMULHW (%_% ymm13) (%_% ymm6) (%_% ymm3) *)
+  0xc5; 0x5d; 0xe5; 0xf3;  (* VPMULHW (%_% ymm14) (%_% ymm4) (%_% ymm3) *)
+  0xc5; 0xa5; 0xf9; 0xff;  (* VPSUBW (%_% ymm7) (%_% ymm11) (%_% ymm7) *)
+  0xc4; 0x41; 0x1d; 0xf9; 0xc9;
+                           (* VPSUBW (%_% ymm9) (%_% ymm12) (%_% ymm9) *)
+  0xc4; 0x41; 0x3d; 0xf9; 0xc5;
+                           (* VPSUBW (%_% ymm8) (%_% ymm8) (%_% ymm13) *)
+  0xc4; 0x41; 0x0d; 0xf9; 0xd2;
+                           (* VPSUBW (%_% ymm10) (%_% ymm14) (%_% ymm10) *)
+  0xc5; 0xbd; 0xfd; 0xff;  (* VPADDW (%_% ymm7) (%_% ymm8) (%_% ymm7) *)
+  0xc4; 0x41; 0x2d; 0xfd; 0xc9;
+                           (* VPADDW (%_% ymm9) (%_% ymm10) (%_% ymm9) *)
+  0xc5; 0x7d; 0x6f; 0x87; 0xc0; 0x00; 0x00; 0x00;
+                           (* VMOVDQA (%_% ymm8) (Memop Word256 (%% (rdi,192))) *)
+  0xc5; 0x7d; 0x6f; 0x97; 0xe0; 0x00; 0x00; 0x00;
+                           (* VMOVDQA (%_% ymm10) (Memop Word256 (%% (rdi,224))) *)
+  0xc5; 0xbd; 0xfd; 0xff;  (* VPADDW (%_% ymm7) (%_% ymm8) (%_% ymm7) *)
+  0xc4; 0x41; 0x2d; 0xfd; 0xc9;
+                           (* VPADDW (%_% ymm9) (%_% ymm10) (%_% ymm9) *)
+  0xc5; 0xfd; 0x7f; 0xbf; 0xc0; 0x00; 0x00; 0x00;
+                           (* VMOVDQA (Memop Word256 (%% (rdi,192))) (%_% ymm7) *)
+  0xc5; 0x7d; 0x7f; 0x8f; 0xe0; 0x00; 0x00; 0x00;
+                           (* VMOVDQA (Memop Word256 (%% (rdi,224))) (%_% ymm9) *)
+  0xc5; 0xfd; 0x6f; 0x96; 0x00; 0x03; 0x00; 0x00;
+                           (* VMOVDQA (%_% ymm2) (Memop Word256 (%% (rsi,768))) *)
+  0xc5; 0xfd; 0x6f; 0x9e; 0x20; 0x03; 0x00; 0x00;
+                           (* VMOVDQA (%_% ymm3) (Memop Word256 (%% (rsi,800))) *)
+  0xc5; 0xfd; 0x6f; 0xa2; 0x00; 0x03; 0x00; 0x00;
+                           (* VMOVDQA (%_% ymm4) (Memop Word256 (%% (rdx,768))) *)
+  0xc5; 0xfd; 0x6f; 0xaa; 0x20; 0x03; 0x00; 0x00;
+                           (* VMOVDQA (%_% ymm5) (Memop Word256 (%% (rdx,800))) *)
+  0xc5; 0xfd; 0x6f; 0xb1; 0x80; 0x01; 0x00; 0x00;
+                           (* VMOVDQA (%_% ymm6) (Memop Word256 (%% (rcx,384))) *)
+  0xc5; 0x75; 0xd5; 0xea;  (* VPMULLW (%_% ymm13) (%_% ymm1) (%_% ymm2) *)
+  0xc5; 0x75; 0xd5; 0xf3;  (* VPMULLW (%_% ymm14) (%_% ymm1) (%_% ymm3) *)
+  0xc4; 0xc1; 0x5d; 0xd5; 0xfd;
+                           (* VPMULLW (%_% ymm7) (%_% ymm4) (%_% ymm13) *)
+  0xc4; 0x41; 0x55; 0xd5; 0xcd;
+                           (* VPMULLW (%_% ymm9) (%_% ymm5) (%_% ymm13) *)
+  0xc4; 0x41; 0x4d; 0xd5; 0xc6;
+                           (* VPMULLW (%_% ymm8) (%_% ymm6) (%_% ymm14) *)
+  0xc4; 0x41; 0x5d; 0xd5; 0xd6;
+                           (* VPMULLW (%_% ymm10) (%_% ymm4) (%_% ymm14) *)
+  0xc5; 0xfd; 0xe5; 0xff;  (* VPMULHW (%_% ymm7) (%_% ymm0) (%_% ymm7) *)
+  0xc4; 0x41; 0x7d; 0xe5; 0xc9;
+                           (* VPMULHW (%_% ymm9) (%_% ymm0) (%_% ymm9) *)
+  0xc4; 0x41; 0x7d; 0xe5; 0xc0;
+                           (* VPMULHW (%_% ymm8) (%_% ymm0) (%_% ymm8) *)
+  0xc4; 0x41; 0x7d; 0xe5; 0xd2;
+                           (* VPMULHW (%_% ymm10) (%_% ymm0) (%_% ymm10) *)
+  0xc5; 0x5d; 0xe5; 0xda;  (* VPMULHW (%_% ymm11) (%_% ymm4) (%_% ymm2) *)
+  0xc5; 0x55; 0xe5; 0xe2;  (* VPMULHW (%_% ymm12) (%_% ymm5) (%_% ymm2) *)
+  0xc5; 0x4d; 0xe5; 0xeb;  (* VPMULHW (%_% ymm13) (%_% ymm6) (%_% ymm3) *)
+  0xc5; 0x5d; 0xe5; 0xf3;  (* VPMULHW (%_% ymm14) (%_% ymm4) (%_% ymm3) *)
+  0xc5; 0xa5; 0xf9; 0xff;  (* VPSUBW (%_% ymm7) (%_% ymm11) (%_% ymm7) *)
+  0xc4; 0x41; 0x1d; 0xf9; 0xc9;
+                           (* VPSUBW (%_% ymm9) (%_% ymm12) (%_% ymm9) *)
+  0xc4; 0x41; 0x15; 0xf9; 0xc0;
+                           (* VPSUBW (%_% ymm8) (%_% ymm13) (%_% ymm8) *)
+  0xc4; 0x41; 0x0d; 0xf9; 0xd2;
+                           (* VPSUBW (%_% ymm10) (%_% ymm14) (%_% ymm10) *)
+  0xc5; 0xbd; 0xfd; 0xff;  (* VPADDW (%_% ymm7) (%_% ymm8) (%_% ymm7) *)
+  0xc4; 0x41; 0x2d; 0xfd; 0xc9;
+                           (* VPADDW (%_% ymm9) (%_% ymm10) (%_% ymm9) *)
+  0xc5; 0x7d; 0x6f; 0x87; 0x00; 0x01; 0x00; 0x00;
+                           (* VMOVDQA (%_% ymm8) (Memop Word256 (%% (rdi,256))) *)
+  0xc5; 0x7d; 0x6f; 0x97; 0x20; 0x01; 0x00; 0x00;
+                           (* VMOVDQA (%_% ymm10) (Memop Word256 (%% (rdi,288))) *)
+  0xc5; 0xbd; 0xfd; 0xff;  (* VPADDW (%_% ymm7) (%_% ymm8) (%_% ymm7) *)
+  0xc4; 0x41; 0x2d; 0xfd; 0xc9;
+                           (* VPADDW (%_% ymm9) (%_% ymm10) (%_% ymm9) *)
+  0xc5; 0xfd; 0x7f; 0xbf; 0x00; 0x01; 0x00; 0x00;
+                           (* VMOVDQA (Memop Word256 (%% (rdi,256))) (%_% ymm7) *)
+  0xc5; 0x7d; 0x7f; 0x8f; 0x20; 0x01; 0x00; 0x00;
+                           (* VMOVDQA (Memop Word256 (%% (rdi,288))) (%_% ymm9) *)
+  0xc5; 0xfd; 0x6f; 0x96; 0x40; 0x03; 0x00; 0x00;
+                           (* VMOVDQA (%_% ymm2) (Memop Word256 (%% (rsi,832))) *)
+  0xc5; 0xfd; 0x6f; 0x9e; 0x60; 0x03; 0x00; 0x00;
+                           (* VMOVDQA (%_% ymm3) (Memop Word256 (%% (rsi,864))) *)
+  0xc5; 0xfd; 0x6f; 0xa2; 0x40; 0x03; 0x00; 0x00;
+                           (* VMOVDQA (%_% ymm4) (Memop Word256 (%% (rdx,832))) *)
+  0xc5; 0xfd; 0x6f; 0xaa; 0x60; 0x03; 0x00; 0x00;
+                           (* VMOVDQA (%_% ymm5) (Memop Word256 (%% (rdx,864))) *)
+  0xc5; 0xfd; 0x6f; 0xb1; 0xa0; 0x01; 0x00; 0x00;
+                           (* VMOVDQA (%_% ymm6) (Memop Word256 (%% (rcx,416))) *)
+  0xc5; 0x75; 0xd5; 0xea;  (* VPMULLW (%_% ymm13) (%_% ymm1) (%_% ymm2) *)
+  0xc5; 0x75; 0xd5; 0xf3;  (* VPMULLW (%_% ymm14) (%_% ymm1) (%_% ymm3) *)
+  0xc4; 0xc1; 0x5d; 0xd5; 0xfd;
+                           (* VPMULLW (%_% ymm7) (%_% ymm4) (%_% ymm13) *)
+  0xc4; 0x41; 0x55; 0xd5; 0xcd;
+                           (* VPMULLW (%_% ymm9) (%_% ymm5) (%_% ymm13) *)
+  0xc4; 0x41; 0x4d; 0xd5; 0xc6;
+                           (* VPMULLW (%_% ymm8) (%_% ymm6) (%_% ymm14) *)
+  0xc4; 0x41; 0x5d; 0xd5; 0xd6;
+                           (* VPMULLW (%_% ymm10) (%_% ymm4) (%_% ymm14) *)
+  0xc5; 0xfd; 0xe5; 0xff;  (* VPMULHW (%_% ymm7) (%_% ymm0) (%_% ymm7) *)
+  0xc4; 0x41; 0x7d; 0xe5; 0xc9;
+                           (* VPMULHW (%_% ymm9) (%_% ymm0) (%_% ymm9) *)
+  0xc4; 0x41; 0x7d; 0xe5; 0xc0;
+                           (* VPMULHW (%_% ymm8) (%_% ymm0) (%_% ymm8) *)
+  0xc4; 0x41; 0x7d; 0xe5; 0xd2;
+                           (* VPMULHW (%_% ymm10) (%_% ymm0) (%_% ymm10) *)
+  0xc5; 0x5d; 0xe5; 0xda;  (* VPMULHW (%_% ymm11) (%_% ymm4) (%_% ymm2) *)
+  0xc5; 0x55; 0xe5; 0xe2;  (* VPMULHW (%_% ymm12) (%_% ymm5) (%_% ymm2) *)
+  0xc5; 0x4d; 0xe5; 0xeb;  (* VPMULHW (%_% ymm13) (%_% ymm6) (%_% ymm3) *)
+  0xc5; 0x5d; 0xe5; 0xf3;  (* VPMULHW (%_% ymm14) (%_% ymm4) (%_% ymm3) *)
+  0xc5; 0xa5; 0xf9; 0xff;  (* VPSUBW (%_% ymm7) (%_% ymm11) (%_% ymm7) *)
+  0xc4; 0x41; 0x1d; 0xf9; 0xc9;
+                           (* VPSUBW (%_% ymm9) (%_% ymm12) (%_% ymm9) *)
+  0xc4; 0x41; 0x3d; 0xf9; 0xc5;
+                           (* VPSUBW (%_% ymm8) (%_% ymm8) (%_% ymm13) *)
+  0xc4; 0x41; 0x0d; 0xf9; 0xd2;
+                           (* VPSUBW (%_% ymm10) (%_% ymm14) (%_% ymm10) *)
+  0xc5; 0xbd; 0xfd; 0xff;  (* VPADDW (%_% ymm7) (%_% ymm8) (%_% ymm7) *)
+  0xc4; 0x41; 0x2d; 0xfd; 0xc9;
+                           (* VPADDW (%_% ymm9) (%_% ymm10) (%_% ymm9) *)
+  0xc5; 0x7d; 0x6f; 0x87; 0x40; 0x01; 0x00; 0x00;
+                           (* VMOVDQA (%_% ymm8) (Memop Word256 (%% (rdi,320))) *)
+  0xc5; 0x7d; 0x6f; 0x97; 0x60; 0x01; 0x00; 0x00;
+                           (* VMOVDQA (%_% ymm10) (Memop Word256 (%% (rdi,352))) *)
+  0xc5; 0xbd; 0xfd; 0xff;  (* VPADDW (%_% ymm7) (%_% ymm8) (%_% ymm7) *)
+  0xc4; 0x41; 0x2d; 0xfd; 0xc9;
+                           (* VPADDW (%_% ymm9) (%_% ymm10) (%_% ymm9) *)
+  0xc5; 0xfd; 0x7f; 0xbf; 0x40; 0x01; 0x00; 0x00;
+                           (* VMOVDQA (Memop Word256 (%% (rdi,320))) (%_% ymm7) *)
+  0xc5; 0x7d; 0x7f; 0x8f; 0x60; 0x01; 0x00; 0x00;
+                           (* VMOVDQA (Memop Word256 (%% (rdi,352))) (%_% ymm9) *)
+  0xc5; 0xfd; 0x6f; 0x96; 0x80; 0x03; 0x00; 0x00;
+                           (* VMOVDQA (%_% ymm2) (Memop Word256 (%% (rsi,896))) *)
+  0xc5; 0xfd; 0x6f; 0x9e; 0xa0; 0x03; 0x00; 0x00;
+                           (* VMOVDQA (%_% ymm3) (Memop Word256 (%% (rsi,928))) *)
+  0xc5; 0xfd; 0x6f; 0xa2; 0x80; 0x03; 0x00; 0x00;
+                           (* VMOVDQA (%_% ymm4) (Memop Word256 (%% (rdx,896))) *)
+  0xc5; 0xfd; 0x6f; 0xaa; 0xa0; 0x03; 0x00; 0x00;
+                           (* VMOVDQA (%_% ymm5) (Memop Word256 (%% (rdx,928))) *)
+  0xc5; 0xfd; 0x6f; 0xb1; 0xc0; 0x01; 0x00; 0x00;
+                           (* VMOVDQA (%_% ymm6) (Memop Word256 (%% (rcx,448))) *)
+  0xc5; 0x75; 0xd5; 0xea;  (* VPMULLW (%_% ymm13) (%_% ymm1) (%_% ymm2) *)
+  0xc5; 0x75; 0xd5; 0xf3;  (* VPMULLW (%_% ymm14) (%_% ymm1) (%_% ymm3) *)
+  0xc4; 0xc1; 0x5d; 0xd5; 0xfd;
+                           (* VPMULLW (%_% ymm7) (%_% ymm4) (%_% ymm13) *)
+  0xc4; 0x41; 0x55; 0xd5; 0xcd;
+                           (* VPMULLW (%_% ymm9) (%_% ymm5) (%_% ymm13) *)
+  0xc4; 0x41; 0x4d; 0xd5; 0xc6;
+                           (* VPMULLW (%_% ymm8) (%_% ymm6) (%_% ymm14) *)
+  0xc4; 0x41; 0x5d; 0xd5; 0xd6;
+                           (* VPMULLW (%_% ymm10) (%_% ymm4) (%_% ymm14) *)
+  0xc5; 0xfd; 0xe5; 0xff;  (* VPMULHW (%_% ymm7) (%_% ymm0) (%_% ymm7) *)
+  0xc4; 0x41; 0x7d; 0xe5; 0xc9;
+                           (* VPMULHW (%_% ymm9) (%_% ymm0) (%_% ymm9) *)
+  0xc4; 0x41; 0x7d; 0xe5; 0xc0;
+                           (* VPMULHW (%_% ymm8) (%_% ymm0) (%_% ymm8) *)
+  0xc4; 0x41; 0x7d; 0xe5; 0xd2;
+                           (* VPMULHW (%_% ymm10) (%_% ymm0) (%_% ymm10) *)
+  0xc5; 0x5d; 0xe5; 0xda;  (* VPMULHW (%_% ymm11) (%_% ymm4) (%_% ymm2) *)
+  0xc5; 0x55; 0xe5; 0xe2;  (* VPMULHW (%_% ymm12) (%_% ymm5) (%_% ymm2) *)
+  0xc5; 0x4d; 0xe5; 0xeb;  (* VPMULHW (%_% ymm13) (%_% ymm6) (%_% ymm3) *)
+  0xc5; 0x5d; 0xe5; 0xf3;  (* VPMULHW (%_% ymm14) (%_% ymm4) (%_% ymm3) *)
+  0xc5; 0xa5; 0xf9; 0xff;  (* VPSUBW (%_% ymm7) (%_% ymm11) (%_% ymm7) *)
+  0xc4; 0x41; 0x1d; 0xf9; 0xc9;
+                           (* VPSUBW (%_% ymm9) (%_% ymm12) (%_% ymm9) *)
+  0xc4; 0x41; 0x15; 0xf9; 0xc0;
+                           (* VPSUBW (%_% ymm8) (%_% ymm13) (%_% ymm8) *)
+  0xc4; 0x41; 0x0d; 0xf9; 0xd2;
+                           (* VPSUBW (%_% ymm10) (%_% ymm14) (%_% ymm10) *)
+  0xc5; 0xbd; 0xfd; 0xff;  (* VPADDW (%_% ymm7) (%_% ymm8) (%_% ymm7) *)
+  0xc4; 0x41; 0x2d; 0xfd; 0xc9;
+                           (* VPADDW (%_% ymm9) (%_% ymm10) (%_% ymm9) *)
+  0xc5; 0x7d; 0x6f; 0x87; 0x80; 0x01; 0x00; 0x00;
+                           (* VMOVDQA (%_% ymm8) (Memop Word256 (%% (rdi,384))) *)
+  0xc5; 0x7d; 0x6f; 0x97; 0xa0; 0x01; 0x00; 0x00;
+                           (* VMOVDQA (%_% ymm10) (Memop Word256 (%% (rdi,416))) *)
+  0xc5; 0xbd; 0xfd; 0xff;  (* VPADDW (%_% ymm7) (%_% ymm8) (%_% ymm7) *)
+  0xc4; 0x41; 0x2d; 0xfd; 0xc9;
+                           (* VPADDW (%_% ymm9) (%_% ymm10) (%_% ymm9) *)
+  0xc5; 0xfd; 0x7f; 0xbf; 0x80; 0x01; 0x00; 0x00;
+                           (* VMOVDQA (Memop Word256 (%% (rdi,384))) (%_% ymm7) *)
+  0xc5; 0x7d; 0x7f; 0x8f; 0xa0; 0x01; 0x00; 0x00;
+                           (* VMOVDQA (Memop Word256 (%% (rdi,416))) (%_% ymm9) *)
+  0xc5; 0xfd; 0x6f; 0x96; 0xc0; 0x03; 0x00; 0x00;
+                           (* VMOVDQA (%_% ymm2) (Memop Word256 (%% (rsi,960))) *)
+  0xc5; 0xfd; 0x6f; 0x9e; 0xe0; 0x03; 0x00; 0x00;
+                           (* VMOVDQA (%_% ymm3) (Memop Word256 (%% (rsi,992))) *)
+  0xc5; 0xfd; 0x6f; 0xa2; 0xc0; 0x03; 0x00; 0x00;
+                           (* VMOVDQA (%_% ymm4) (Memop Word256 (%% (rdx,960))) *)
+  0xc5; 0xfd; 0x6f; 0xaa; 0xe0; 0x03; 0x00; 0x00;
+                           (* VMOVDQA (%_% ymm5) (Memop Word256 (%% (rdx,992))) *)
+  0xc5; 0xfd; 0x6f; 0xb1; 0xe0; 0x01; 0x00; 0x00;
+                           (* VMOVDQA (%_% ymm6) (Memop Word256 (%% (rcx,480))) *)
+  0xc5; 0x75; 0xd5; 0xea;  (* VPMULLW (%_% ymm13) (%_% ymm1) (%_% ymm2) *)
+  0xc5; 0x75; 0xd5; 0xf3;  (* VPMULLW (%_% ymm14) (%_% ymm1) (%_% ymm3) *)
+  0xc4; 0xc1; 0x5d; 0xd5; 0xfd;
+                           (* VPMULLW (%_% ymm7) (%_% ymm4) (%_% ymm13) *)
+  0xc4; 0x41; 0x55; 0xd5; 0xcd;
+                           (* VPMULLW (%_% ymm9) (%_% ymm5) (%_% ymm13) *)
+  0xc4; 0x41; 0x4d; 0xd5; 0xc6;
+                           (* VPMULLW (%_% ymm8) (%_% ymm6) (%_% ymm14) *)
+  0xc4; 0x41; 0x5d; 0xd5; 0xd6;
+                           (* VPMULLW (%_% ymm10) (%_% ymm4) (%_% ymm14) *)
+  0xc5; 0xfd; 0xe5; 0xff;  (* VPMULHW (%_% ymm7) (%_% ymm0) (%_% ymm7) *)
+  0xc4; 0x41; 0x7d; 0xe5; 0xc9;
+                           (* VPMULHW (%_% ymm9) (%_% ymm0) (%_% ymm9) *)
+  0xc4; 0x41; 0x7d; 0xe5; 0xc0;
+                           (* VPMULHW (%_% ymm8) (%_% ymm0) (%_% ymm8) *)
+  0xc4; 0x41; 0x7d; 0xe5; 0xd2;
+                           (* VPMULHW (%_% ymm10) (%_% ymm0) (%_% ymm10) *)
+  0xc5; 0x5d; 0xe5; 0xda;  (* VPMULHW (%_% ymm11) (%_% ymm4) (%_% ymm2) *)
+  0xc5; 0x55; 0xe5; 0xe2;  (* VPMULHW (%_% ymm12) (%_% ymm5) (%_% ymm2) *)
+  0xc5; 0x4d; 0xe5; 0xeb;  (* VPMULHW (%_% ymm13) (%_% ymm6) (%_% ymm3) *)
+  0xc5; 0x5d; 0xe5; 0xf3;  (* VPMULHW (%_% ymm14) (%_% ymm4) (%_% ymm3) *)
+  0xc5; 0xa5; 0xf9; 0xff;  (* VPSUBW (%_% ymm7) (%_% ymm11) (%_% ymm7) *)
+  0xc4; 0x41; 0x1d; 0xf9; 0xc9;
+                           (* VPSUBW (%_% ymm9) (%_% ymm12) (%_% ymm9) *)
+  0xc4; 0x41; 0x3d; 0xf9; 0xc5;
+                           (* VPSUBW (%_% ymm8) (%_% ymm8) (%_% ymm13) *)
+  0xc4; 0x41; 0x0d; 0xf9; 0xd2;
+                           (* VPSUBW (%_% ymm10) (%_% ymm14) (%_% ymm10) *)
+  0xc5; 0xbd; 0xfd; 0xff;  (* VPADDW (%_% ymm7) (%_% ymm8) (%_% ymm7) *)
+  0xc4; 0x41; 0x2d; 0xfd; 0xc9;
+                           (* VPADDW (%_% ymm9) (%_% ymm10) (%_% ymm9) *)
+  0xc5; 0x7d; 0x6f; 0x87; 0xc0; 0x01; 0x00; 0x00;
+                           (* VMOVDQA (%_% ymm8) (Memop Word256 (%% (rdi,448))) *)
+  0xc5; 0x7d; 0x6f; 0x97; 0xe0; 0x01; 0x00; 0x00;
+                           (* VMOVDQA (%_% ymm10) (Memop Word256 (%% (rdi,480))) *)
+  0xc5; 0xbd; 0xfd; 0xff;  (* VPADDW (%_% ymm7) (%_% ymm8) (%_% ymm7) *)
+  0xc4; 0x41; 0x2d; 0xfd; 0xc9;
+                           (* VPADDW (%_% ymm9) (%_% ymm10) (%_% ymm9) *)
+  0xc5; 0xfd; 0x7f; 0xbf; 0xc0; 0x01; 0x00; 0x00;
+                           (* VMOVDQA (Memop Word256 (%% (rdi,448))) (%_% ymm7) *)
+  0xc5; 0x7d; 0x7f; 0x8f; 0xe0; 0x01; 0x00; 0x00;
+                           (* VMOVDQA (Memop Word256 (%% (rdi,480))) (%_% ymm9) *)
+  0xc3                     (* RET *)
+];;
+
+let mlkem_basemul_k2_tmc = define_trimmed "mlkem_basemul_k2_tmc" mlkem_basemul_k2_mc;;
+let mlkem_basemul_k2_tmc_EXEC = X86_MK_CORE_EXEC_RULE mlkem_basemul_k2_tmc;;
+
+(* Enable simplification of word_subwords by default.
+   Nedded to prevent the symbolic simulation to explode
+   as we add more instructions. *)
+let org_extra_word_conv = !extra_word_CONV;;
+extra_word_CONV := [WORD_SIMPLE_SUBWORD_CONV] @ !extra_word_CONV;;
+
+
+(* (a + bX) * (c + dX) = (a*c + b*dz) + (a*d + b*c)X *)
+let pmul0 = define
+  `pmul0 (a: int) (b : int) (c : int) (dz : int) = b*dz + a*c`;;
+
+let pmul0_odd = define
+  `pmul0_odd (a: int) (b : int) (c : int) (dz : int) = a*c - b*dz`;;
+
+let pmul1 = define
+  `pmul1 (a: int) (b : int) (c : int) (d : int) = b*c + a*d`;;
+
+let pmulacc0 = define
+  `pmulacc0 (a0: int) (b0 : int) (c0 : int) (d0 : int) (dz0 : int)
+            (a1: int) (b1 : int) (c1 : int) (d1 : int) (dz1 : int) =
+              pmul0 a0 b0 c0 dz0 + pmul0 a1 b1 c1 dz1`;;
+
+let pmulacc0_odd = define
+  `pmulacc0_odd (a0: int) (b0 : int) (c0 : int) (d0 : int) (dz0 : int)
+                (a1: int) (b1 : int) (c1 : int) (d1 : int) (dz1 : int) =
+              pmul0_odd a0 b0 c0 dz0 + pmul0_odd a1 b1 c1 dz1`;;
+
+let pmulacc1 = define
+  `pmulacc1 (a0: int) (b0 : int) (c0 : int) (d0 : int) (dz0 : int)
+            (a1: int) (b1 : int) (c1 : int) (d1 : int) (dz1 : int) =
+              pmul1 a0 b0 c0 d0 + pmul1 a1 b1 c1 d1`;;
+
+let pmulaccred0 = define
+  `pmulaccred0 (a0: int) (b0 : int) (c0 : int) (d0 : int) (dz0 : int)
+               (a1: int) (b1 : int) (c1 : int) (d1 : int) (dz1 : int) =
+     (&(inverse_mod 3329 65536) * pmulacc0 a0 b0 c0 d0 dz0 a1 b1 c1 d1 dz1) rem &3329`;;
+
+let pmulaccred0_odd = define
+  `pmulaccred0_odd (a0: int) (b0 : int) (c0 : int) (d0 : int) (dz0 : int)
+                   (a1: int) (b1 : int) (c1 : int) (d1 : int) (dz1 : int) =
+     (&(inverse_mod 3329 65536) * pmulacc0_odd a0 b0 c0 d0 dz0 a1 b1 c1 d1 dz1) rem &3329`;;
+
+
+let pmulaccred1 = define
+  `pmulaccred1 (a0: int) (b0 : int) (c0 : int) (d0 : int) (dz0 : int)
+               (a1: int) (b1 : int) (c1 : int) (d1 : int) (dz1 : int) =
+     (&(inverse_mod 3329 65536) * pmulacc1 a0 b0 c0 d0 dz0 a1 b1 c1 d1 dz1) rem &3329`;;
+
+let MLKEM_BASEMUL_K2_CORRECT = prove(
+  `!src1 src2 src2t dst a0 b0 c0 d0 dz0 a1 b1 c1 d1 dz1 pc.
+        aligned 32 src1 /\
+        aligned 32 src2 /\
+        aligned 32 src2t /\
+        aligned 32 dst /\
+        ALL (nonoverlapping (dst, 512)) [(src1, 1024); (src2, 1024); (src2t, 512)] /\
+        nonoverlapping (dst, 512) (word pc, 2502)
+        ==> ensures x86
+              (\s. bytes_loaded s (word pc) (BUTLAST mlkem_basemul_k2_tmc) /\
+                   read RIP s = word pc /\
+                   C_ARGUMENTS [dst; src1; src2; src2t] s /\
+                   (!i. i < 16 ==> !j. j < 8
+                        ==> read(memory :> bytes16
+                             (word_add src1 (word (64*j + 2*i)))) s = a0 i j) /\
+                   (!i. i < 16 ==> !j. j < 8
+                        ==> read(memory :> bytes16
+                             (word_add src1 (word (64*j + 32 + 2*i)))) s = b0 i j) /\
+                   (!i. i < 16 ==> !j. j < 8
+                        ==> read(memory :> bytes16
+                             (word_add src2 (word (64*j + 2*i)))) s = c0 i j) /\
+                   (!i. i < 16 ==> !j. j < 8
+                        ==> read(memory :> bytes16
+                             (word_add src2 (word (64*j + 32 + 2*i)))) s = d0 i j) /\
+                   (!i. i < 16 ==> !j. j < 8
+                        ==> read(memory :> bytes16
+                             (word_add src2t (word (32*j + 2*i)))) s = dz0 i j) /\
+                             
+                   (!i. i < 16 ==> !j. j < 8
+                        ==> read(memory :> bytes16
+                             (word_add src1 (word (512 + 64*j + 2*i)))) s = a1 i j) /\
+                   (!i. i < 16 ==> !j. j < 8
+                        ==> read(memory :> bytes16
+                             (word_add src1 (word (512 + 64*j + 32 + 2*i)))) s = b1 i j) /\
+                   (!i. i < 16 ==> !j. j < 8
+                        ==> read(memory :> bytes16
+                             (word_add src2 (word (512 + 64*j + 2*i)))) s = c1 i j) /\
+                   (!i. i < 16 ==> !j. j < 8
+                        ==> read(memory :> bytes16
+                             (word_add src2 (word (512 + 64*j + 32 + 2*i)))) s = d1 i j) /\
+                   (!i. i < 16 ==> !j. j < 8
+                        ==> read(memory :> bytes16
+                             (word_add src2t (word (256 + 32*j + 2*i)))) s = dz1 i j))
+              (\s. read RIP s = word (pc + 2502) /\
+                   (!i. i < 16 ==> !j. j < 4
+                        ==> (let j' = 2*j in
+                              (abs(ival(a0 i j')) <= &2 pow 12  /\
+                               abs(ival(b0 i j')) <= &2 pow 12  /\
+                               abs(ival(a1 i j')) <= &2 pow 12  /\
+                               abs(ival(b1 i j')) <= &2 pow 12
+                               ==>
+                               (ival (read(memory :> bytes16 (word_add dst (word (64*j' + 2*i)))) s)
+                                ==
+                                pmulaccred0 (ival (a0 i j')) (ival (b0 i j')) (ival (c0 i j')) (ival (d0 i j')) (ival (dz0 i j'))
+                                            (ival (a1 i j')) (ival (b1 i j')) (ival (c1 i j')) (ival (d1 i j')) (ival (dz1 i j'))
+                               ) (mod &3329)))) /\
+
+                   (!i. i < 16 ==> !j. j < 4
+                        ==> (let j' = 2*j+1 in
+                              (abs(ival(a0 i j')) <= &2 pow 12  /\
+                               abs(ival(b0 i j')) <= &2 pow 12  /\
+                               abs(ival(a1 i j')) <= &2 pow 12  /\
+                               abs(ival(b1 i j')) <= &2 pow 12
+                               ==>
+                               (ival (read(memory :> bytes16 (word_add dst (word (64*j' + 2*i)))) s)
+                                ==
+                                pmulaccred0_odd (ival (a0 i j')) (ival (b0 i j')) (ival (c0 i j')) (ival (d0 i j')) (ival (dz0 i j'))
+                                            (ival (a1 i j')) (ival (b1 i j')) (ival (c1 i j')) (ival (d1 i j')) (ival (dz1 i j'))
+                               ) (mod &3329)))) /\
+
+                   (!i. i < 16 ==> !j. j < 8
+                        ==> abs(ival(a0 i j)) <= &2 pow 12  /\
+                            abs(ival(b0 i j)) <= &2 pow 12  /\
+                            abs(ival(a1 i j)) <= &2 pow 12  /\
+                            abs(ival(b1 i j)) <= &2 pow 12
+                        ==> (ival (read(memory :> bytes16 (word_add dst (word (64*j + 32 + 2*i)))) s)
+                             ==
+                             pmulaccred1 (ival (a0 i j)) (ival (b0 i j)) (ival (c0 i j)) (ival (d0 i j)) (ival (dz0 i j))
+                                         (ival (a1 i j)) (ival (b1 i j)) (ival (c1 i j)) (ival (d1 i j)) (ival (dz1 i j))
+                            ) (mod &3329)))
+              (MAYCHANGE [events] ,,
+               MAYCHANGE [RIP] ,, MAYCHANGE [RAX] ,,
+               MAYCHANGE [ZMM0; ZMM1; ZMM2; ZMM3; ZMM4; ZMM5; ZMM6; ZMM7;
+                          ZMM8; ZMM9; ZMM10; ZMM11; ZMM12; ZMM13; ZMM14] ,,
+               MAYCHANGE [memory :> bytes(dst, 512)])`,
+
+  REWRITE_TAC [MAYCHANGE_REGS_AND_FLAGS_PERMITTED_BY_ABI;
+    NONOVERLAPPING_CLAUSES; ALL; C_ARGUMENTS; fst mlkem_basemul_k2_tmc_EXEC] THEN
+  REPEAT STRIP_TAC THEN
+
+  GHOST_INTRO_TAC `init_ymm0:int256` `read YMM0` THEN
+  GHOST_INTRO_TAC `init_ymm1:int256` `read YMM1` THEN
+
+  CONV_TAC(RATOR_CONV(LAND_CONV(TOP_DEPTH_CONV EXPAND_CASES_CONV))) THEN
+  CONV_TAC(TOP_DEPTH_CONV NUM_MULT_CONV THENC
+           TOP_DEPTH_CONV NUM_ADD_CONV) THEN
+
+  ENSURES_INIT_TAC "s0" THEN
+
+  MEMORY_256_FROM_16_TAC "src1" 64 THEN
+  MEMORY_256_FROM_16_TAC "src2" 64 THEN
+  MEMORY_256_FROM_16_TAC "src2t" 32 THEN
+
+  ASM_REWRITE_TAC [WORD_ADD_0] THEN
+  DISCARD_MATCHING_ASSUMPTIONS [`read (memory :> bytes16 any) s = x`] THEN
+  REPEAT STRIP_TAC THEN
+
+  MAP_EVERY (fun n -> X86_STEPS_TAC mlkem_basemul_k2_tmc_EXEC [n] THEN
+                      SIMD_SIMPLIFY_TAC [montmul_x86; montmul_odd_x86])
+            (1--470) THEN
+
+  ENSURES_FINAL_STATE_TAC THEN
+  ASM_REWRITE_TAC[] THEN
+
+  REPEAT(FIRST_X_ASSUM(STRIP_ASSUME_TAC o
+  CONV_RULE(SIMD_SIMPLIFY_CONV[]) o
+  CONV_RULE(READ_MEMORY_SPLIT_CONV 4) o
+  check (can (term_match [] `read qqq s:int256 = xxx`) o concl))) THEN
+
+  CONV_TAC(TOP_DEPTH_CONV EXPAND_CASES_CONV) THEN
+  CONV_TAC(DEPTH_CONV NUM_MULT_CONV THENC
+           DEPTH_CONV NUM_ADD_CONV THENC
+           DEPTH_CONV let_CONV) THEN
+  CONV_TAC(DEPTH_CONV NUM_MULT_CONV THENC
+           DEPTH_CONV NUM_ADD_CONV THENC
+           DEPTH_CONV let_CONV) THEN
+  ASM_REWRITE_TAC[WORD_ADD_0] THEN
+
+  DISCARD_STATE_TAC "s470" THEN
+
+  REPEAT CONJ_TAC THEN
+  REWRITE_TAC[pmulaccred0; pmulacc0; pmul0; pmulaccred0_odd;
+              pmulacc0_odd; pmul0_odd; pmulaccred1; pmulacc1; pmul1] THEN
+  STRIP_TAC THEN
+  ASSUM_LIST((fun ths -> W(MP_TAC o CONJUNCT1 o GEN_CONGBOUND_RULE ths o
+    rand o lhand o rator o snd))) THEN
+  REWRITE_TAC[GSYM INT_REM_EQ] THEN CONV_TAC INT_REM_DOWN_CONV THEN
+  MATCH_MP_TAC EQ_IMP THEN AP_TERM_TAC THEN AP_THM_TAC THEN AP_TERM_TAC THEN
+  CONV_TAC INT_RING
+);;
+
+let MLKEM_BASEMUL_K2_NOIBT_SUBROUTINE_CORRECT = prove(
+  `!src1 src2 src2t dst a0 b0 c0 d0 dz0 a1 b1 c1 d1 dz1 pc stackpointer returnaddress.
+        aligned 32 src1 /\
+        aligned 32 src2 /\
+        aligned 32 src2t /\
+        aligned 32 dst /\
+        ALL (nonoverlapping (dst, 512)) [(src1, 1024); (src2, 1024); (src2t, 512)] /\
+        nonoverlapping (dst, 512) (word pc, LENGTH mlkem_basemul_k2_tmc) /\
+        nonoverlapping (dst, 512) (stackpointer, 8)
+        ==> ensures x86
+              (\s. bytes_loaded s (word pc) mlkem_basemul_k2_tmc /\
+                   read RIP s = word pc /\
+                   read RSP s = stackpointer /\
+                   read (memory :> bytes64 stackpointer) s = returnaddress /\
+                   C_ARGUMENTS [dst; src1; src2; src2t] s /\
+                   (!i. i < 16 ==> !j. j < 8
+                        ==> read(memory :> bytes16
+                             (word_add src1 (word (64*j + 2*i)))) s = a0 i j) /\
+                   (!i. i < 16 ==> !j. j < 8
+                        ==> read(memory :> bytes16
+                             (word_add src1 (word (64*j + 32 + 2*i)))) s = b0 i j) /\
+                   (!i. i < 16 ==> !j. j < 8
+                        ==> read(memory :> bytes16
+                             (word_add src2 (word (64*j + 2*i)))) s = c0 i j) /\
+                   (!i. i < 16 ==> !j. j < 8
+                        ==> read(memory :> bytes16
+                             (word_add src2 (word (64*j + 32 + 2*i)))) s = d0 i j) /\
+                   (!i. i < 16 ==> !j. j < 8
+                        ==> read(memory :> bytes16
+                             (word_add src2t (word (32*j + 2*i)))) s = dz0 i j) /\
+                             
+                   (!i. i < 16 ==> !j. j < 8
+                        ==> read(memory :> bytes16
+                             (word_add src1 (word (512 + 64*j + 2*i)))) s = a1 i j) /\
+                   (!i. i < 16 ==> !j. j < 8
+                        ==> read(memory :> bytes16
+                             (word_add src1 (word (512 + 64*j + 32 + 2*i)))) s = b1 i j) /\
+                   (!i. i < 16 ==> !j. j < 8
+                        ==> read(memory :> bytes16
+                             (word_add src2 (word (512 + 64*j + 2*i)))) s = c1 i j) /\
+                   (!i. i < 16 ==> !j. j < 8
+                        ==> read(memory :> bytes16
+                             (word_add src2 (word (512 + 64*j + 32 + 2*i)))) s = d1 i j) /\
+                   (!i. i < 16 ==> !j. j < 8
+                        ==> read(memory :> bytes16
+                             (word_add src2t (word (256 + 32*j + 2*i)))) s = dz1 i j))
+              (\s. read RIP s = returnaddress /\
+                   read RSP s = word_add stackpointer (word 8) /\
+                   (!i. i < 16 ==> !j. j < 4
+                        ==> (let j' = 2*j in
+                              (abs(ival(a0 i j')) <= &2 pow 12  /\
+                               abs(ival(b0 i j')) <= &2 pow 12  /\
+                               abs(ival(a1 i j')) <= &2 pow 12  /\
+                               abs(ival(b1 i j')) <= &2 pow 12
+                               ==>
+                               (ival (read(memory :> bytes16 (word_add dst (word (64*j' + 2*i)))) s)
+                                ==
+                                pmulaccred0 (ival (a0 i j')) (ival (b0 i j')) (ival (c0 i j')) (ival (d0 i j')) (ival (dz0 i j'))
+                                            (ival (a1 i j')) (ival (b1 i j')) (ival (c1 i j')) (ival (d1 i j')) (ival (dz1 i j'))
+                               ) (mod &3329)))) /\
+
+                   (!i. i < 16 ==> !j. j < 4
+                        ==> (let j' = 2*j+1 in
+                              (abs(ival(a0 i j')) <= &2 pow 12  /\
+                               abs(ival(b0 i j')) <= &2 pow 12  /\
+                               abs(ival(a1 i j')) <= &2 pow 12  /\
+                               abs(ival(b1 i j')) <= &2 pow 12
+                               ==>
+                               (ival (read(memory :> bytes16 (word_add dst (word (64*j' + 2*i)))) s)
+                                ==
+                                pmulaccred0_odd (ival (a0 i j')) (ival (b0 i j')) (ival (c0 i j')) (ival (d0 i j')) (ival (dz0 i j'))
+                                            (ival (a1 i j')) (ival (b1 i j')) (ival (c1 i j')) (ival (d1 i j')) (ival (dz1 i j'))
+                               ) (mod &3329)))) /\
+
+                   (!i. i < 16 ==> !j. j < 8
+                        ==> abs(ival(a0 i j)) <= &2 pow 12  /\
+                            abs(ival(b0 i j)) <= &2 pow 12  /\
+                            abs(ival(a1 i j)) <= &2 pow 12  /\
+                            abs(ival(b1 i j)) <= &2 pow 12
+                        ==> (ival (read(memory :> bytes16 (word_add dst (word (64*j + 32 + 2*i)))) s)
+                             ==
+                             pmulaccred1 (ival (a0 i j)) (ival (b0 i j)) (ival (c0 i j)) (ival (d0 i j)) (ival (dz0 i j))
+                                         (ival (a1 i j)) (ival (b1 i j)) (ival (c1 i j)) (ival (d1 i j)) (ival (dz1 i j))
+                            ) (mod &3329)))
+              (MAYCHANGE [RSP] ,, MAYCHANGE_REGS_AND_FLAGS_PERMITTED_BY_ABI ,,
+               MAYCHANGE [memory :> bytes(dst, 512)])`,
+  X86_PROMOTE_RETURN_NOSTACK_TAC mlkem_basemul_k2_tmc MLKEM_BASEMUL_K2_CORRECT);;
+
+let MLKEM_BASEMUL_K2_SUBROUTINE_CORRECT = prove(
+  `!src1 src2 src2t dst a0 b0 c0 d0 dz0 a1 b1 c1 d1 dz1 pc stackpointer returnaddress.
+        aligned 32 src1 /\
+        aligned 32 src2 /\
+        aligned 32 src2t /\
+        aligned 32 dst /\
+        ALL (nonoverlapping (dst, 512)) [(src1, 1024); (src2, 1024); (src2t, 512)] /\
+        nonoverlapping (dst, 512) (word pc, LENGTH mlkem_basemul_k2_mc) /\
+        nonoverlapping (dst, 512) (stackpointer, 8)
+        ==> ensures x86
+              (\s. bytes_loaded s (word pc) mlkem_basemul_k2_mc /\
+                   read RIP s = word pc /\
+                   read RSP s = stackpointer /\
+                   read (memory :> bytes64 stackpointer) s = returnaddress /\
+                   C_ARGUMENTS [dst; src1; src2; src2t] s /\
+                   (!i. i < 16 ==> !j. j < 8
+                        ==> read(memory :> bytes16
+                             (word_add src1 (word (64*j + 2*i)))) s = a0 i j) /\
+                   (!i. i < 16 ==> !j. j < 8
+                        ==> read(memory :> bytes16
+                             (word_add src1 (word (64*j + 32 + 2*i)))) s = b0 i j) /\
+                   (!i. i < 16 ==> !j. j < 8
+                        ==> read(memory :> bytes16
+                             (word_add src2 (word (64*j + 2*i)))) s = c0 i j) /\
+                   (!i. i < 16 ==> !j. j < 8
+                        ==> read(memory :> bytes16
+                             (word_add src2 (word (64*j + 32 + 2*i)))) s = d0 i j) /\
+                   (!i. i < 16 ==> !j. j < 8
+                        ==> read(memory :> bytes16
+                             (word_add src2t (word (32*j + 2*i)))) s = dz0 i j) /\
+                             
+                   (!i. i < 16 ==> !j. j < 8
+                        ==> read(memory :> bytes16
+                             (word_add src1 (word (512 + 64*j + 2*i)))) s = a1 i j) /\
+                   (!i. i < 16 ==> !j. j < 8
+                        ==> read(memory :> bytes16
+                             (word_add src1 (word (512 + 64*j + 32 + 2*i)))) s = b1 i j) /\
+                   (!i. i < 16 ==> !j. j < 8
+                        ==> read(memory :> bytes16
+                             (word_add src2 (word (512 + 64*j + 2*i)))) s = c1 i j) /\
+                   (!i. i < 16 ==> !j. j < 8
+                        ==> read(memory :> bytes16
+                             (word_add src2 (word (512 + 64*j + 32 + 2*i)))) s = d1 i j) /\
+                   (!i. i < 16 ==> !j. j < 8
+                        ==> read(memory :> bytes16
+                             (word_add src2t (word (256 + 32*j + 2*i)))) s = dz1 i j))
+              (\s. read RIP s = returnaddress /\
+                   read RSP s = word_add stackpointer (word 8) /\
+                   (!i. i < 16 ==> !j. j < 4
+                        ==> (let j' = 2*j in
+                              (abs(ival(a0 i j')) <= &2 pow 12  /\
+                               abs(ival(b0 i j')) <= &2 pow 12  /\
+                               abs(ival(a1 i j')) <= &2 pow 12  /\
+                               abs(ival(b1 i j')) <= &2 pow 12
+                               ==>
+                               (ival (read(memory :> bytes16 (word_add dst (word (64*j' + 2*i)))) s)
+                                ==
+                                pmulaccred0 (ival (a0 i j')) (ival (b0 i j')) (ival (c0 i j')) (ival (d0 i j')) (ival (dz0 i j'))
+                                            (ival (a1 i j')) (ival (b1 i j')) (ival (c1 i j')) (ival (d1 i j')) (ival (dz1 i j'))
+                               ) (mod &3329)))) /\
+
+                   (!i. i < 16 ==> !j. j < 4
+                        ==> (let j' = 2*j+1 in
+                              (abs(ival(a0 i j')) <= &2 pow 12  /\
+                               abs(ival(b0 i j')) <= &2 pow 12  /\
+                               abs(ival(a1 i j')) <= &2 pow 12  /\
+                               abs(ival(b1 i j')) <= &2 pow 12
+                               ==>
+                               (ival (read(memory :> bytes16 (word_add dst (word (64*j' + 2*i)))) s)
+                                ==
+                                pmulaccred0_odd (ival (a0 i j')) (ival (b0 i j')) (ival (c0 i j')) (ival (d0 i j')) (ival (dz0 i j'))
+                                            (ival (a1 i j')) (ival (b1 i j')) (ival (c1 i j')) (ival (d1 i j')) (ival (dz1 i j'))
+                               ) (mod &3329)))) /\
+
+                   (!i. i < 16 ==> !j. j < 8
+                        ==> abs(ival(a0 i j)) <= &2 pow 12  /\
+                            abs(ival(b0 i j)) <= &2 pow 12  /\
+                            abs(ival(a1 i j)) <= &2 pow 12  /\
+                            abs(ival(b1 i j)) <= &2 pow 12
+                        ==> (ival (read(memory :> bytes16 (word_add dst (word (64*j + 32 + 2*i)))) s)
+                             ==
+                             pmulaccred1 (ival (a0 i j)) (ival (b0 i j)) (ival (c0 i j)) (ival (d0 i j)) (ival (dz0 i j))
+                                         (ival (a1 i j)) (ival (b1 i j)) (ival (c1 i j)) (ival (d1 i j)) (ival (dz1 i j))
+                            ) (mod &3329)))
+              (MAYCHANGE [RSP] ,, MAYCHANGE_REGS_AND_FLAGS_PERMITTED_BY_ABI ,,
+               MAYCHANGE [memory :> bytes(dst, 512)])`,
+  MATCH_ACCEPT_TAC(ADD_IBT_RULE MLKEM_BASEMUL_K2_NOIBT_SUBROUTINE_CORRECT));;
+
+
+(* ------------------------------------------------------------------------- *)
+(* Correctness of Windows ABI version.                                       *)
+(* ------------------------------------------------------------------------- *)
+
+let mlkem_basemul_k2_windows_mc = define_from_elf
+    "mlkem_basemul_k2_windows_mc" "x86/mlkem/mlkem_basemul_k2.obj";;
+
+let mlkem_basemul_k2_windows_tmc = define_trimmed
+    "mlkem_basemul_k2_windows_tmc" mlkem_basemul_k2_windows_mc;;
+
+let mlkem_basemul_k2_windows_tmc_EXEC = X86_MK_EXEC_RULE mlkem_basemul_k2_windows_tmc;;
+
+let MLKEM_BASEMUL_K2_NOIBT_WINDOWS_SUBROUTINE_CORRECT = prove(
+  `!src1 src2 src2t dst a0 b0 c0 d0 dz0 a1 b1 c1 d1 dz1 pc stackpointer returnaddress.
+        aligned 32 src1 /\
+        aligned 32 src2 /\
+        aligned 32 src2t /\
+        aligned 32 dst /\
+        nonoverlapping (word pc, LENGTH mlkem_basemul_k2_windows_tmc)
+                       (word_sub stackpointer (word 176), 176) /\
+        nonoverlapping (src1, 1024)
+                       (word_sub stackpointer (word 176), 176) /\
+        nonoverlapping (src2, 1024)
+                       (word_sub stackpointer (word 176), 176) /\
+        nonoverlapping (src2t, 512)
+                       (word_sub stackpointer (word 176), 176) /\
+        nonoverlapping (dst, 512) (src1, 1024) /\
+        nonoverlapping (dst, 512) (src2, 1024) /\
+        nonoverlapping (dst, 512) (src2t, 512) /\
+        nonoverlapping (dst, 512) (src2t, 512) /\
+        nonoverlapping (dst, 512) (word pc, LENGTH mlkem_basemul_k2_windows_tmc) /\
+        nonoverlapping (dst, 512) (word_sub stackpointer (word 176), 184)
+        ==> ensures x86 
+              (\s. bytes_loaded s (word pc) mlkem_basemul_k2_windows_tmc /\
+                   read RIP s = word pc /\
+                   read RSP s = stackpointer /\
+                   read (memory :> bytes64 stackpointer) s = returnaddress /\
+                   WINDOWS_C_ARGUMENTS [dst; src1; src2; src2t] s /\
+                   (!i. i < 16 ==> !j. j < 8
+                        ==> read(memory :> bytes16
+                             (word_add src1 (word (64*j + 2*i)))) s = a0 i j) /\
+                   (!i. i < 16 ==> !j. j < 8
+                        ==> read(memory :> bytes16
+                             (word_add src1 (word (64*j + 32 + 2*i)))) s = b0 i j) /\
+                   (!i. i < 16 ==> !j. j < 8
+                        ==> read(memory :> bytes16
+                             (word_add src2 (word (64*j + 2*i)))) s = c0 i j) /\
+                   (!i. i < 16 ==> !j. j < 8
+                        ==> read(memory :> bytes16
+                             (word_add src2 (word (64*j + 32 + 2*i)))) s = d0 i j) /\
+                   (!i. i < 16 ==> !j. j < 8
+                        ==> read(memory :> bytes16
+                             (word_add src2t (word (32*j + 2*i)))) s = dz0 i j) /\
+                             
+                   (!i. i < 16 ==> !j. j < 8
+                        ==> read(memory :> bytes16
+                             (word_add src1 (word (512 + 64*j + 2*i)))) s = a1 i j) /\
+                   (!i. i < 16 ==> !j. j < 8
+                        ==> read(memory :> bytes16
+                             (word_add src1 (word (512 + 64*j + 32 + 2*i)))) s = b1 i j) /\
+                   (!i. i < 16 ==> !j. j < 8
+                        ==> read(memory :> bytes16
+                             (word_add src2 (word (512 + 64*j + 2*i)))) s = c1 i j) /\
+                   (!i. i < 16 ==> !j. j < 8
+                        ==> read(memory :> bytes16
+                             (word_add src2 (word (512 + 64*j + 32 + 2*i)))) s = d1 i j) /\
+                   (!i. i < 16 ==> !j. j < 8
+                        ==> read(memory :> bytes16
+                             (word_add src2t (word (256 + 32*j + 2*i)))) s = dz1 i j))
+              (\s. read RIP s = returnaddress /\
+                   read RSP s = word_add stackpointer (word 8) /\
+                   (!i. i < 16 ==> !j. j < 4
+                        ==> (let j' = 2*j in
+                              (abs(ival(a0 i j')) <= &2 pow 12  /\
+                               abs(ival(b0 i j')) <= &2 pow 12  /\
+                               abs(ival(a1 i j')) <= &2 pow 12  /\
+                               abs(ival(b1 i j')) <= &2 pow 12
+                               ==>
+                               (ival (read(memory :> bytes16 (word_add dst (word (64*j' + 2*i)))) s)
+                                ==
+                                pmulaccred0 (ival (a0 i j')) (ival (b0 i j')) (ival (c0 i j')) (ival (d0 i j')) (ival (dz0 i j'))
+                                            (ival (a1 i j')) (ival (b1 i j')) (ival (c1 i j')) (ival (d1 i j')) (ival (dz1 i j'))
+                               ) (mod &3329)))) /\
+
+                   (!i. i < 16 ==> !j. j < 4
+                        ==> (let j' = 2*j+1 in
+                              (abs(ival(a0 i j')) <= &2 pow 12  /\
+                               abs(ival(b0 i j')) <= &2 pow 12  /\
+                               abs(ival(a1 i j')) <= &2 pow 12  /\
+                               abs(ival(b1 i j')) <= &2 pow 12
+                               ==>
+                               (ival (read(memory :> bytes16 (word_add dst (word (64*j' + 2*i)))) s)
+                                ==
+                                pmulaccred0_odd (ival (a0 i j')) (ival (b0 i j')) (ival (c0 i j')) (ival (d0 i j')) (ival (dz0 i j'))
+                                            (ival (a1 i j')) (ival (b1 i j')) (ival (c1 i j')) (ival (d1 i j')) (ival (dz1 i j'))
+                               ) (mod &3329)))) /\
+
+                   (!i. i < 16 ==> !j. j < 8
+                        ==> abs(ival(a0 i j)) <= &2 pow 12  /\
+                            abs(ival(b0 i j)) <= &2 pow 12  /\
+                            abs(ival(a1 i j)) <= &2 pow 12  /\
+                            abs(ival(b1 i j)) <= &2 pow 12
+                        ==> (ival (read(memory :> bytes16 (word_add dst (word (64*j + 32 + 2*i)))) s)
+                             ==
+                             pmulaccred1 (ival (a0 i j)) (ival (b0 i j)) (ival (c0 i j)) (ival (d0 i j)) (ival (dz0 i j))
+                                         (ival (a1 i j)) (ival (b1 i j)) (ival (c1 i j)) (ival (d1 i j)) (ival (dz1 i j))
+                            ) (mod &3329)))
+              (MAYCHANGE [RSP] ,, WINDOWS_MAYCHANGE_REGS_AND_FLAGS_PERMITTED_BY_ABI ,,
+               MAYCHANGE [memory :> bytes(word_sub stackpointer (word 176), 176)] ,,
+               MAYCHANGE [memory :> bytes(dst, 512)])`,
+  REPLICATE_TAC 15 GEN_TAC THEN
+  WORD_FORALL_OFFSET_TAC 176 THEN
+  REPEAT GEN_TAC THEN
+
+  REWRITE_TAC[fst mlkem_basemul_k2_windows_tmc_EXEC] THEN
+  REPEAT STRIP_TAC THEN REWRITE_TAC[ALL; WINDOWS_C_ARGUMENTS] THEN
+  REWRITE_TAC[WINDOWS_MAYCHANGE_REGS_AND_FLAGS_PERMITTED_BY_ABI] THEN
+
+  ENSURES_PRESERVED_TAC "rdi_init" `RDI` THEN
+  ENSURES_PRESERVED_TAC "rsi_init" `RSI` THEN
+  ENSURES_PRESERVED_TAC "init_xmm6" `ZMM6 :> bottomhalf :> bottomhalf` THEN
+  ENSURES_PRESERVED_TAC "init_xmm7" `ZMM7 :> bottomhalf :> bottomhalf` THEN
+  ENSURES_PRESERVED_TAC "init_xmm8" `ZMM8 :> bottomhalf :> bottomhalf` THEN
+  ENSURES_PRESERVED_TAC "init_xmm9" `ZMM9 :> bottomhalf :> bottomhalf` THEN
+  ENSURES_PRESERVED_TAC "init_xmm10" `ZMM10 :> bottomhalf :> bottomhalf` THEN
+  ENSURES_PRESERVED_TAC "init_xmm11" `ZMM11 :> bottomhalf :> bottomhalf` THEN
+  ENSURES_PRESERVED_TAC "init_xmm12" `ZMM12 :> bottomhalf :> bottomhalf` THEN
+  ENSURES_PRESERVED_TAC "init_xmm13" `ZMM13 :> bottomhalf :> bottomhalf` THEN
+  ENSURES_PRESERVED_TAC "init_xmm14" `ZMM14 :> bottomhalf :> bottomhalf` THEN
+
+  REWRITE_TAC[READ_ZMM_BOTTOM_QUARTER'] THEN
+  REWRITE_TAC(map GSYM
+    [YMM6;YMM7;YMM8;YMM9;YMM10;YMM11;YMM12;YMM13;YMM14]) THEN
+
+  GHOST_INTRO_TAC `init_ymm6:int256` `read YMM6` THEN
+  GHOST_INTRO_TAC `init_ymm7:int256` `read YMM7` THEN
+  GHOST_INTRO_TAC `init_ymm8:int256` `read YMM8` THEN
+  GHOST_INTRO_TAC `init_ymm9:int256` `read YMM9` THEN
+  GHOST_INTRO_TAC `init_ymm10:int256` `read YMM10` THEN
+  GHOST_INTRO_TAC `init_ymm11:int256` `read YMM11` THEN
+  GHOST_INTRO_TAC `init_ymm12:int256` `read YMM12` THEN
+  GHOST_INTRO_TAC `init_ymm13:int256` `read YMM13` THEN
+  GHOST_INTRO_TAC `init_ymm14:int256` `read YMM14` THEN
+
+  GLOBALIZE_PRECONDITION_TAC THEN
+  REPEAT(FIRST_X_ASSUM(SUBST1_TAC o SYM)) THEN
+
+  ENSURES_INIT_TAC "s0" THEN
+  X86_STEPS_TAC mlkem_basemul_k2_windows_tmc_EXEC (1--18) THEN
+
+  MP_TAC(SPECL [`src1:int64`; `src2:int64`; `src2t:int64`; `dst:int64`;
+                `a0:num->num->int16`; `b0:num->num->int16`; `c0:num->num->int16`; `d0:num->num->int16`; `dz0:num->num->int16`;
+                `a1:num->num->int16`; `b1:num->num->int16`; `c1:num->num->int16`; `d1:num->num->int16`; `dz1:num->num->int16`;
+                `pc + 105`] MLKEM_BASEMUL_K2_CORRECT) THEN
+  ASM_REWRITE_TAC[C_ARGUMENTS; SOME_FLAGS] THEN REWRITE_TAC[ALL] THEN
+  ANTS_TAC THENL [NONOVERLAPPING_TAC; ALL_TAC] THEN
+
+  X86_BIGSTEP_TAC mlkem_basemul_k2_windows_tmc_EXEC "s19" THENL
+   [FIRST_ASSUM(MATCH_ACCEPT_TAC o MATCH_MP
+     (BYTES_LOADED_SUBPROGRAM_RULE mlkem_basemul_k2_windows_tmc
+     (REWRITE_RULE[BUTLAST_CLAUSES]
+      (AP_TERM `BUTLAST:byte list->byte list` mlkem_basemul_k2_tmc))
+     105));
+    RULE_ASSUM_TAC(CONV_RULE(TRY_CONV RIP_PLUS_CONV))] THEN
+
+    
+  MAP_EVERY ABBREV_TAC
+   [`ymm6_epilog = read YMM6 s19`;
+    `ymm7_epilog = read YMM7 s19`;
+    `ymm8_epilog = read YMM8 s19`;
+    `ymm9_epilog = read YMM9 s19`;
+    `ymm10_epilog = read YMM10 s19`;
+    `ymm11_epilog = read YMM11 s19`;
+    `ymm12_epilog = read YMM12 s19`;
+    `ymm13_epilog = read YMM13 s19`;
+    `ymm14_epilog = read YMM14 s19`] THEN
+
+  X86_STEPS_TAC mlkem_basemul_k2_windows_tmc_EXEC (20--34) THEN
+
+  RULE_ASSUM_TAC(REWRITE_RULE[MAYCHANGE_ZMM_QUARTER]) THEN
+  RULE_ASSUM_TAC(REWRITE_RULE[MAYCHANGE_YMM_SSE_QUARTER]) THEN
+
+  ENSURES_FINAL_STATE_TAC THEN ASM_REWRITE_TAC[] THEN
+  REPEAT CONJ_TAC THEN CONV_TAC WORD_BLAST
+);;
+
+
+let MLKEM_BASEMUL_K2_WINDOWS_SUBROUTINE_CORRECT = prove(
+  `!src1 src2 src2t dst a0 b0 c0 d0 dz0 a1 b1 c1 d1 dz1 pc stackpointer returnaddress.
+        aligned 32 src1 /\
+        aligned 32 src2 /\
+        aligned 32 src2t /\
+        aligned 32 dst /\
+        nonoverlapping (word pc, LENGTH mlkem_basemul_k2_windows_mc)
+                       (word_sub stackpointer (word 176), 176) /\
+        nonoverlapping (src1, 1024)
+                       (word_sub stackpointer (word 176), 176) /\
+        nonoverlapping (src2, 1024)
+                       (word_sub stackpointer (word 176), 176) /\
+        nonoverlapping (src2t, 512)
+                       (word_sub stackpointer (word 176), 176) /\
+        nonoverlapping (dst, 512) (src1, 1024) /\
+        nonoverlapping (dst, 512) (src2, 1024) /\
+        nonoverlapping (dst, 512) (src2t, 512) /\
+        nonoverlapping (dst, 512) (src2t, 512) /\
+        nonoverlapping (dst, 512) (word pc, LENGTH mlkem_basemul_k2_windows_mc) /\
+        nonoverlapping (dst, 512) (word_sub stackpointer (word 176), 184)
+        ==> ensures x86 
+              (\s. bytes_loaded s (word pc) mlkem_basemul_k2_windows_mc /\
+                   read RIP s = word pc /\
+                   read RSP s = stackpointer /\
+                   read (memory :> bytes64 stackpointer) s = returnaddress /\
+                   WINDOWS_C_ARGUMENTS [dst; src1; src2; src2t] s /\
+                   (!i. i < 16 ==> !j. j < 8
+                        ==> read(memory :> bytes16
+                             (word_add src1 (word (64*j + 2*i)))) s = a0 i j) /\
+                   (!i. i < 16 ==> !j. j < 8
+                        ==> read(memory :> bytes16
+                             (word_add src1 (word (64*j + 32 + 2*i)))) s = b0 i j) /\
+                   (!i. i < 16 ==> !j. j < 8
+                        ==> read(memory :> bytes16
+                             (word_add src2 (word (64*j + 2*i)))) s = c0 i j) /\
+                   (!i. i < 16 ==> !j. j < 8
+                        ==> read(memory :> bytes16
+                             (word_add src2 (word (64*j + 32 + 2*i)))) s = d0 i j) /\
+                   (!i. i < 16 ==> !j. j < 8
+                        ==> read(memory :> bytes16
+                             (word_add src2t (word (32*j + 2*i)))) s = dz0 i j) /\
+                             
+                   (!i. i < 16 ==> !j. j < 8
+                        ==> read(memory :> bytes16
+                             (word_add src1 (word (512 + 64*j + 2*i)))) s = a1 i j) /\
+                   (!i. i < 16 ==> !j. j < 8
+                        ==> read(memory :> bytes16
+                             (word_add src1 (word (512 + 64*j + 32 + 2*i)))) s = b1 i j) /\
+                   (!i. i < 16 ==> !j. j < 8
+                        ==> read(memory :> bytes16
+                             (word_add src2 (word (512 + 64*j + 2*i)))) s = c1 i j) /\
+                   (!i. i < 16 ==> !j. j < 8
+                        ==> read(memory :> bytes16
+                             (word_add src2 (word (512 + 64*j + 32 + 2*i)))) s = d1 i j) /\
+                   (!i. i < 16 ==> !j. j < 8
+                        ==> read(memory :> bytes16
+                             (word_add src2t (word (256 + 32*j + 2*i)))) s = dz1 i j))
+              (\s. read RIP s = returnaddress /\
+                   read RSP s = word_add stackpointer (word 8) /\
+                   (!i. i < 16 ==> !j. j < 4
+                        ==> (let j' = 2*j in
+                              (abs(ival(a0 i j')) <= &2 pow 12  /\
+                               abs(ival(b0 i j')) <= &2 pow 12  /\
+                               abs(ival(a1 i j')) <= &2 pow 12  /\
+                               abs(ival(b1 i j')) <= &2 pow 12
+                               ==>
+                               (ival (read(memory :> bytes16 (word_add dst (word (64*j' + 2*i)))) s)
+                                ==
+                                pmulaccred0 (ival (a0 i j')) (ival (b0 i j')) (ival (c0 i j')) (ival (d0 i j')) (ival (dz0 i j'))
+                                            (ival (a1 i j')) (ival (b1 i j')) (ival (c1 i j')) (ival (d1 i j')) (ival (dz1 i j'))
+                               ) (mod &3329)))) /\
+
+                   (!i. i < 16 ==> !j. j < 4
+                        ==> (let j' = 2*j+1 in
+                              (abs(ival(a0 i j')) <= &2 pow 12  /\
+                               abs(ival(b0 i j')) <= &2 pow 12  /\
+                               abs(ival(a1 i j')) <= &2 pow 12  /\
+                               abs(ival(b1 i j')) <= &2 pow 12
+                               ==>
+                               (ival (read(memory :> bytes16 (word_add dst (word (64*j' + 2*i)))) s)
+                                ==
+                                pmulaccred0_odd (ival (a0 i j')) (ival (b0 i j')) (ival (c0 i j')) (ival (d0 i j')) (ival (dz0 i j'))
+                                            (ival (a1 i j')) (ival (b1 i j')) (ival (c1 i j')) (ival (d1 i j')) (ival (dz1 i j'))
+                               ) (mod &3329)))) /\
+
+                   (!i. i < 16 ==> !j. j < 8
+                        ==> abs(ival(a0 i j)) <= &2 pow 12  /\
+                            abs(ival(b0 i j)) <= &2 pow 12  /\
+                            abs(ival(a1 i j)) <= &2 pow 12  /\
+                            abs(ival(b1 i j)) <= &2 pow 12
+                        ==> (ival (read(memory :> bytes16 (word_add dst (word (64*j + 32 + 2*i)))) s)
+                             ==
+                             pmulaccred1 (ival (a0 i j)) (ival (b0 i j)) (ival (c0 i j)) (ival (d0 i j)) (ival (dz0 i j))
+                                         (ival (a1 i j)) (ival (b1 i j)) (ival (c1 i j)) (ival (d1 i j)) (ival (dz1 i j))
+                            ) (mod &3329)))
+              (MAYCHANGE [RSP] ,, WINDOWS_MAYCHANGE_REGS_AND_FLAGS_PERMITTED_BY_ABI ,,
+               MAYCHANGE [memory :> bytes(word_sub stackpointer (word 176), 176)] ,,
+               MAYCHANGE [memory :> bytes(dst, 512)])`,
+  MATCH_ACCEPT_TAC(ADD_IBT_RULE MLKEM_BASEMUL_K2_NOIBT_WINDOWS_SUBROUTINE_CORRECT));;
